src/Bedrock/Group/CurveAdd/LoopBody.v
@@ -1,6 +1,6 @@
 Require Import Rupicola.Lib.Api. Import bedrock2.WeakestPrecondition.
 Require Import Crypto.Arithmetic.PrimeFieldTheorems.
-Require Import Crypto.Bedrock.Group.CurveAdd.StoreZeroGSpec.
+Require Import Crypto.Bedrock.Group.CurveAdd.StoreZero.
 Require Import Crypto.Bedrock.Specs.Field.
 Require Import Crypto.Bedrock.Field.Interface.CompilationAbstract.
 Require Import Crypto.Bedrock.Group.CurveAdd.CurveAddAlt.
@@ -28,6 +28,7 @@ Section __.
           {field_representation_ok : FieldRepresentation_ok F}
           {group_cmov : string}
           {store_zero : string}.
+  Context {scalar_words : nat}.
 
   Hint Resolve relax_bounds : compiler.
   Existing Instance felem_alloc.
@@ -35,43 +36,60 @@ Section __.
   (* Proof. *)
   (*     exact field_representation. *)
   (* Defined. *)
+  Context (curve_add_name : string).
 
   Context (Hbounds_eq : loose_bounds = tight_bounds).
   Context (three_b : felem).
   Context (Hb_bounds : maybe_bounded (Some loose_bounds) three_b).
 
-  Instance spec_of_curve_add : spec_of "ladderstep" := spec_of_curve_add_alt three_b.
+  Instance spec_of_curve_add : spec_of curve_add_name := spec_of_curve_add_alt three_b.
 
-  Instance spec_of_bignum_shift : spec_of "shift_scalar" := spec_of_shift_scalar.
+  Instance spec_of_bignum_shift : spec_of "shift_scalar" := spec_of_shift_scalar (scalar_words:=scalar_words).
 
   Instance spec_of_cond_move : spec_of "group_cmov" := spec_of_group_cmov.
+  Instance spec_of_cond_move_alt : spec_of "group_cmov_alt" := spec_of_group_cmov_alt.
 
-  Instance spec_of_store_zero : spec_of "store_zero_G" := spec_of_store_zero.
+  Instance spec_of_store_zero : spec_of "store_zero" := spec_of_store_zero.
 
-  Context {n_init : Z}
-          {Px_init Py_init Pz_init : F}
-          {curve_add : (F * F * F) -> (F * F * F) -> (F * F * F)}.
+  (* this should all be generalized: F * F * F should be a generic group etc. *)
+  Context
+    {n_init : Z}
+      {Px_init Py_init Pz_init : F}
+      {curve_add : (F * F * F) -> (F * F * F) -> (F * F * F)}
+      {curve_add_assoc : forall P Q R, curve_add P (curve_add Q R) = curve_add (curve_add P Q) R}
+      (* NB: both of these are used, and they hold in all groups,
+         so we assume both rather than commutativity, since it is not necessary *)
+      {curve_add_zero_l : forall P, curve_add (Fzero, Fone, Fzero) P = P}
+      {curve_add_zero_r : forall P, curve_add P (Fzero, Fone, Fzero) = P}.
 
-          Fixpoint scmul (n : nat)  : F * F * F -> F * F * F :=
-            fun (P : F * F * F) =>
-              let X := (fst (fst P) ) in
-              let Y := (snd (fst P)) in
-              let Z := (snd P) in
-            match n with
-            | O => (Fzero, Fone, Fzero)
-            | S m => curve_add (X, Y, Z) (scmul m (X, Y, Z))
-            end.
-        
-  Context {group_prop1 : forall x y z a b c n m k,
-        @CurveAdd.ladderstep_gallina _ _ _ _ _ field_parameters field_representation three_b x y z a b c = \<n, m, k\>
-        -> (n, m, k) = curve_add (x, y, z) (a, b, c)}
-        {group_prop2 : forall x y z n m k iter xinit yinit zinit,
-        (n, m, k) = curve_add (x, y, z) (x, y, z) ->
-        (x, y, z) = scmul (2 ^ iter) (xinit, yinit, zinit) ->
-        (n, m, k) = scmul (2 ^ (iter + 1)) (xinit, yinit, zinit)}
-        .
+  Fixpoint scmul (n : nat)  : F * F * F -> F * F * F :=
+    fun (P : F * F * F) =>
+      let X := (fst (fst P) ) in
+      let Y := (snd (fst P)) in
+      let Z := (snd P) in
+      match n with
+      | O => (Fzero, Fone, Fzero)
+      | S m => curve_add (X, Y, Z) (scmul m (X, Y, Z))
+      end.
 
-  Context (group_property1 : forall x, curve_add (Fzero, Fone, Fzero) x = x) .
+  Lemma scmul_add n m : forall x y z,
+      scmul (n + m) (x, y, z) = curve_add (scmul n (x, y, z)) (scmul m (x, y, z)).
+  Proof.
+    intros.
+    induction n.
+    - simpl. rewrite curve_add_zero_l. reflexivity.
+    - simpl. rewrite IHn. rewrite curve_add_assoc. reflexivity.
+  Qed.
+
+  Context
+    {curve_add_spec : forall x y z a b c n m k, @CurveAdd.ladderstep_gallina _ _ _ _ _ field_parameters field_representation three_b x a y b z c = \<n, m, k\> -> (n, m, k) = curve_add (x, y, z) (a, b, c)}.
+      (* {group_prop2 : forall x y z n m k iter xinit yinit zinit, *)
+      (*   (n, m, k) = curve_add (x, y, z) (x, y, z) -> *)
+      (*   (x, y, z) = scmul (2 ^ iter) (xinit, yinit, zinit) -> *)
+      (*   (n, m, k) = scmul (2 ^ (iter + 1)) (xinit, yinit, zinit)} *)
+      (*   . *)
+
+  (* Context (group_property1 : forall x, curve_add (Fzero, Fone, Fzero) x = x) . *)
 
   Local Notation bit_range := {|ZRange.lower := 0; ZRange.upper := 1|}.
 
@@ -86,16 +104,16 @@ Section __.
          * FElem (Some tight_bounds) pOutx Outx
          * FElem (Some tight_bounds) pOuty Outy
          * FElem (Some tight_bounds) pOutz Outz
-         * FElem (Some tight_bounds) pPauxx Pauxx
-         * FElem (Some tight_bounds) pPauxy Pauxy
-         * FElem (Some tight_bounds) pPauxz Pauxz
-         * Bignum.Bignum 6 pn n
-         * Bignum.Bignum 1 pc [c]
+         * FElem None pPauxx Pauxx
+         * FElem None pPauxy Pauxy
+         * FElem None pPauxz Pauxz
+         * Bignum.Bignum scalar_words pn n
+         * scalar pc c
          * R)%sep mem
-         /\ (*n*)
-            (Positional.eval (uweight 64) 6 (List.map word.unsigned n)) = Z.shiftr n_init (Z.of_nat iter)
-         /\ (Outx, Outy, Outz) = scmul  (Z.to_nat (n_init mod (2 ^ (Z.of_nat iter))))%Z (Px_init, Py_init, Pz_init)
-         /\ (Px, Py, Pz) = scmul (2 ^ iter) (Px_init, Py_init, Pz_init)
+        (* these bounds should be incorporated in the Bignum.Bignum predicate, as it is in FElem *)
+         /\ (Positional.eval (uweight width) scalar_words (List.map word.unsigned n)) = Z.shiftr n_init (Z.of_nat iter)
+         /\ (Outx, Outy, Outz) = scmul (Z.to_nat (n_init mod (2 ^ (Z.of_nat iter))))%Z (Px_init, Py_init, Pz_init)
+         /\ (Px, Py, Pz) = scmul  (2 ^ iter) (Px_init, Py_init, Pz_init)
          ;
       ensures tr' mem' :=
         tr = tr'
@@ -104,10 +122,9 @@ Section __.
            exists nnew : list word,
            exists cnew : word,
                (*n*)
-               (Positional.eval (uweight 64) 6 (List.map word.unsigned nnew)) = Z.shiftr n_init (Z.of_nat (iter + 1))
+            (Positional.eval (uweight width) scalar_words (List.map word.unsigned nnew)) = Z.shiftr n_init (Z.of_nat (iter + 1))
             /\ (Outxnew, Outynew, Outznew) = scmul  (Z.to_nat (n_init mod (2 ^ (Z.of_nat (iter + 1)))))%Z (Px_init, Py_init, Pz_init)
-            /\ (Pxnew, Pynew, Pznew) = scmul (2 ^ (iter + 1)) (Px_init, Py_init, Pz_init)
-
+            /\ (Pxnew, Pynew, Pznew) = scmul  (2 ^ (iter + 1)) (Px_init, Py_init, Pz_init)
           /\ (FElem (Some tight_bounds) pPx Pxnew
                 * FElem (Some tight_bounds) pPy Pynew
                 * FElem (Some tight_bounds) pPz Pznew
@@ -117,8 +134,8 @@ Section __.
                 * FElem (Some tight_bounds) pPauxx Pauxxnew
                 * FElem (Some tight_bounds) pPauxy Pauxynew
                 * FElem (Some tight_bounds) pPauxz Pauxznew
-                * Bignum.Bignum 6 pn nnew
-                * Bignum.Bignum 1 pc [cnew]
+                * Bignum.Bignum scalar_words pn nnew
+                * scalar pc cnew
                 * R)%sep mem'}.
 
   Require Import bedrock2.NotationsCustomEntry.
@@ -129,635 +146,166 @@ Section __.
 
   Definition loop_body_func : bedrock2.Syntax.func :=
     ("loop_body", (["px"; "py"; "pz"; "outx"; "outy"; "outz"; "pauxx"; "pauxy"; "pauxz"; "pn"; "pc"], []:list String.string, bedrock_func_body:(
-      coq:(cmd.call [] ("store_zero_G") [expr.var ("pauxx"); expr.var ("pauxy"); expr.var ("pauxz")]);
+      coq:(cmd.call [] ("store_zero") [expr.var ("pauxx"); expr.var ("pauxy"); expr.var ("pauxz")]);
       coq:(cmd.call [] ("shift_scalar") [expr.var ("pc"); expr.var ("pn")]);
-      coq:(cmd.call [] ("group_cmov") [expr.var ("pauxx"); expr.var ("pauxy"); expr.var ("pauxz"); expr.var ("pauxx"); expr.var ("pauxy"); expr.var ("pauxz"); expr.var ("px"); expr.var ("py"); expr.var ("pz"); expr.var("pc")]);
-      coq:(cmd.call [] ("ladderstep") [expr.var ("outx"); expr.var ("outy"); expr.var ("outz"); expr.var ("pauxx"); expr.var ("pauxy"); expr.var ("pauxz"); expr.var ("outx"); expr.var ("outy"); expr.var ("outz")]);
-      coq:(cmd.call [] ("ladderstep") [expr.var ("px"); expr.var ("py"); expr.var ("pz"); expr.var ("px"); expr.var ("py"); expr.var ("pz"); expr.var ("px"); expr.var ("py"); expr.var ("pz")])
+      coq:(cmd.call [] ("group_cmov_alt") [expr.var ("pauxx"); expr.var ("pauxy"); expr.var ("pauxz"); expr.var ("pauxx"); expr.var ("pauxy"); expr.var ("pauxz"); expr.var ("px"); expr.var ("py"); expr.var ("pz"); expr.var("pc")]);
+      coq:(cmd.call [] (curve_add_name)
+             [expr.var ("outx");
+              expr.var ("pauxx");
+              expr.var ("outy");
+              expr.var ("pauxy");
+              expr.var ("outz");
+              expr.var ("pauxz");
+              expr.var ("outx");
+              expr.var ("outy");
+              expr.var ("outz")]);
+      coq:(cmd.call [] (curve_add_name)
+             [expr.var ("px");
+              expr.var ("px");
+              expr.var ("py");
+              expr.var ("py");
+              expr.var ("pz");
+              expr.var ("pz");
+              expr.var ("px");
+              expr.var ("py");
+              expr.var ("pz")])
     ))).
 
-    From bedrock2 Require Import ToCString Bytedump.
-    Definition c_mod := (c_module (loop_body_func :: nil)).
-    Eval native_compute in c_mod.
+    (* From bedrock2 Require Import ToCString Bytedump. *)
+    (* Definition c_mod := (c_module (loop_body_func :: nil)). *)
+    (* Eval native_compute in c_mod. *)
 
-    Print c_mod.
+    (* Print c_mod. *)
+
+  Ltac straightline' :=
+    match goal with
+    | |- felem_size_in_bytes mod _ = 0 => eapply felem_size_in_bytes_mod
+    | |- ?a mod ?a = 0 => eapply Z_mod_same_full
+    (* | _ => update_mem *)
+    | _ => straightline
+    | l := _ : map.rep |- _ => subst l
+    | l := _ : list word.rep |- _ => subst l
+    | |- Some _ = Some _ => try reflexivity
+    | |- exists _, _ => eexists
+    | |- _ /\ _ => split
+    | |- map.get _ _ = _ => repeat (erewrite map.get_put_diff; [| intros contra; discriminate]); eapply map.get_put_same
+    end.
 
     Lemma loop_body_ok : program_logic_goal_for_function! loop_body_func.
     Proof.
-      repeat straightline.
-      eexists; split.
-      {
-        repeat straightline. eexists. split.
-          - subst l.
-            repeat (erewrite map.get_put_diff; [| intros contra; discriminate]).
-            eapply map.get_put_same.
-          - repeat straightline. eexists. split.
-          {
-            subst l.
-            repeat (erewrite map.get_put_diff; [| intros contra; discriminate]).
-            eapply map.get_put_same.
-          }
-          repeat straightline. eexists. split.
-          {
-            subst l.
-            repeat (erewrite map.get_put_diff; [| intros contra; discriminate]).
-            eapply map.get_put_same.
-          }
-          repeat straightline.
-      }
-      repeat straightline.
-
-      eapply Proper_call.
-      2: {
-        eapply H. ecancel_assumption.
-      }
-      cbv [pointwise_relation Basics.impl].
-      repeat straightline.
-
-      eexists. split.
-      {
-        subst l. repeat straightline. eexists; split.
-        {
-          repeat (erewrite map.get_put_diff; [| intros contra; discriminate]).
-          eapply map.get_put_same.
-        }
-        repeat straightline. eexists; split.
-        {
-          repeat (erewrite map.get_put_diff; [| intros contra; discriminate]).
-          eapply map.get_put_same.
-        }
-        repeat straightline.
-      }
-
-      eapply Proper_call.
-      2: eapply H0; ecancel_assumption.
-
-      cbv [pointwise_relation Basics.impl].
-      repeat straightline.
-
-      eexists. split.
-      {
-        repeat straightline. eexists. split.
-        {
-          subst l.
-          repeat (erewrite map.get_put_diff; [| intros contra; discriminate]).
-          eapply map.get_put_same.
-        }
-        repeat straightline. eexists. split.
-        {
-          subst l.
-          repeat (erewrite map.get_put_diff; [| intros contra; discriminate]).
-          eapply map.get_put_same.
-        }
-        repeat straightline. eexists. split.
-        {
-          subst l.
-          repeat (erewrite map.get_put_diff; [| intros contra; discriminate]).
-          eapply map.get_put_same.
-        }
-        repeat straightline. eexists. split.
-        {
-          subst l.
-          repeat (erewrite map.get_put_diff; [| intros contra; discriminate]).
-          eapply map.get_put_same.
-        }
-        repeat straightline. eexists. split.
-        {
-          subst l.
-          repeat (erewrite map.get_put_diff; [| intros contra; discriminate]).
-          eapply map.get_put_same.
-        }
-        repeat straightline. eexists. split.
-        {
-          subst l.
-          repeat (erewrite map.get_put_diff; [| intros contra; discriminate]).
-          eapply map.get_put_same.
-        }
-        repeat straightline. eexists. split.
-        {
-          subst l.
-          repeat (erewrite map.get_put_diff; [| intros contra; discriminate]).
-          eapply map.get_put_same.
-        }
-        repeat straightline. eexists. split.
-        {
-          subst l.
-          repeat (erewrite map.get_put_diff; [| intros contra; discriminate]).
-          eapply map.get_put_same.
-        }
-        repeat straightline. eexists. split.
-        {
-          subst l.
-          repeat (erewrite map.get_put_diff; [| intros contra; discriminate]).
-          eapply map.get_put_same.
-        }
-        repeat straightline. eexists. split.
-        {
-          subst l.
-          repeat (erewrite map.get_put_diff; [| intros contra; discriminate]).
-          eapply map.get_put_same.
-        }
-        repeat straightline. 
-      }
-
-      assert (length x0 = 1)%nat.
-      {
-        cbv [Bignum.Bignum] in H12. sepsimpl. eauto.
-      }
-      destruct x0; try discriminate.
-      destruct x0; try discriminate.
-
-      Admitted.
-
-    (*   eapply Proper_call. *)
-    (*   2: eapply H1. *)
-    (*   2: { *)
-    (*     (* cbv [my_field_representation] in *. *) *)
-    (*     split. *)
-    (*     ecancel_assumption. *)
-    (*     split; [ecancel_assumption| ]. *)
-    (*     eassert (Positional.eval (uweight 64) 1 [word.unsigned r] = word.unsigned r). *)
-    (*     { *)
-    (*       rewrite Positional.eval_cons; eauto. simpl. *)
-    (*       cbv [uweight ModOps.weight]; simpl. *)
-    (*       rewrite Positional.eval_nil. lia. *)
-    (*     } *)
-    (*     simpl in H11. *)
-    (*     rewrite H13 in H11. *)
-
-    (*     cbv [ZRange.is_bounded_by_bool]. simpl. *)
-    (*     assert (0 <=? word.unsigned r = true). *)
-    (*     { *)
-    (*       rewrite <- H11; lia. *)
-    (*     } *)
-    (*     rewrite H14. *)
-    (*     assert (word.unsigned r <=? 1 = true) by (rewrite <- H11; lia). *)
-    (*     rewrite H15. auto. *)
-    (*   } *)
-
-    (*   cbv [pointwise_relation Basics.impl]. *)
-    (*   repeat straightline. *)
-
-    (*   repeat straightline. eexists. split. *)
-    (*   { *)
-    (*     repeat straightline. eexists. split. *)
-    (*     { *)
-    (*       subst l. *)
-    (*       repeat (erewrite map.get_put_diff; [| intros contra; discriminate]). *)
-    (*       eapply map.get_put_same. *)
-    (*     } *)
-    (*     repeat straightline. eexists. split. *)
-    (*     { *)
-    (*       subst l. *)
-    (*       repeat (erewrite map.get_put_diff; [| intros contra; discriminate]). *)
-    (*       eapply map.get_put_same. *)
-    (*     } *)
-    (*     repeat straightline. eexists. split. *)
-    (*     { *)
-    (*       subst l. *)
-    (*       repeat (erewrite map.get_put_diff; [| intros contra; discriminate]). *)
-    (*       eapply map.get_put_same. *)
-    (*     } *)
-    (*     repeat straightline. eexists. split. *)
-    (*     { *)
-    (*       subst l. *)
-    (*       repeat (erewrite map.get_put_diff; [| intros contra; discriminate]). *)
-    (*       eapply map.get_put_same. *)
-    (*     } *)
-    (*     repeat straightline. eexists. split. *)
-    (*     { *)
-    (*       subst l. *)
-    (*       repeat (erewrite map.get_put_diff; [| intros contra; discriminate]). *)
-    (*       eapply map.get_put_same. *)
-    (*     } *)
-    (*     repeat straightline. eexists. split. *)
-    (*     { *)
-    (*       subst l. *)
-    (*       repeat (erewrite map.get_put_diff; [| intros contra; discriminate]). *)
-    (*       eapply map.get_put_same. *)
-    (*     } *)
-    (*     repeat straightline. eexists. split. *)
-    (*     { *)
-    (*       subst l. *)
-    (*       repeat (erewrite map.get_put_diff; [| intros contra; discriminate]). *)
-    (*       eapply map.get_put_same. *)
-    (*     } *)
-    (*     repeat straightline. eexists. split. *)
-    (*     { *)
-    (*       subst l. *)
-    (*       repeat (erewrite map.get_put_diff; [| intros contra; discriminate]). *)
-    (*       eapply map.get_put_same. *)
-    (*     } *)
-    (*     repeat straightline. eexists. split. *)
-    (*     { *)
-    (*       subst l. *)
-    (*       repeat (erewrite map.get_put_diff; [| intros contra; discriminate]). *)
-    (*       eapply map.get_put_same. *)
-    (*     } *)
-    (*     repeat straightline. *)
-    (*   } *)
-
-    (*   eapply Proper_call. *)
-    (*   2 : { *)
-    (*     eapply H2. *)
-    (*     (* cbv [CurveAddAlt.my_field_representation my_field_representation] in *. *) *)
-    (*     do 2 (try split); ecancel_assumption. *)
-    (*   } *)
-
-    (*   cbv [pointwise_relation Basics.impl]. *)
-    (*   repeat straightline. *)
-
-    (*   eexists. split. *)
-    (*   { *)
-    (*     repeat straightline. eexists. split. *)
-    (*     { *)
-    (*       subst l. *)
-    (*       repeat (erewrite map.get_put_diff; [| intros contra; discriminate]). *)
-    (*       eapply map.get_put_same. *)
-    (*     } *)
-    (*     repeat straightline. eexists. split. *)
-    (*     { *)
-    (*       subst l. *)
-    (*       repeat (erewrite map.get_put_diff; [| intros contra; discriminate]). *)
-    (*       eapply map.get_put_same. *)
-    (*     } *)
-    (*     repeat straightline. eexists. split. *)
-    (*     { *)
-    (*       subst l. *)
-    (*       repeat (erewrite map.get_put_diff; [| intros contra; discriminate]). *)
-    (*       eapply map.get_put_same. *)
-    (*     } *)
-    (*     repeat straightline. eexists. split. *)
-    (*     { *)
-    (*       subst l. *)
-    (*       repeat (erewrite map.get_put_diff; [| intros contra; discriminate]). *)
-    (*       eapply map.get_put_same. *)
-    (*     } *)
-    (*     repeat straightline. eexists. split. *)
-    (*     { *)
-    (*       subst l. *)
-    (*       repeat (erewrite map.get_put_diff; [| intros contra; discriminate]). *)
-    (*       eapply map.get_put_same. *)
-    (*     } *)
-    (*     repeat straightline. eexists. split. *)
-    (*     { *)
-    (*       subst l. *)
-    (*       repeat (erewrite map.get_put_diff; [| intros contra; discriminate]). *)
-    (*       eapply map.get_put_same. *)
-    (*     } *)
-    (*     repeat straightline. eexists. split. *)
-    (*     { *)
-    (*       subst l. *)
-    (*       repeat (erewrite map.get_put_diff; [| intros contra; discriminate]). *)
-    (*       eapply map.get_put_same. *)
-    (*     } *)
-    (*     repeat straightline. eexists. split. *)
-    (*     { *)
-    (*       subst l. *)
-    (*       repeat (erewrite map.get_put_diff; [| intros contra; discriminate]). *)
-    (*       eapply map.get_put_same. *)
-    (*     } *)
-    (*     repeat straightline. eexists. split. *)
-    (*     { *)
-    (*       subst l. *)
-    (*       repeat (erewrite map.get_put_diff; [| intros contra; discriminate]). *)
-    (*       eapply map.get_put_same. *)
-    (*     } *)
-    (*     repeat straightline. *)
-    (*   } *)
-    (*   eapply Proper_call. *)
-
-    (*   2: { *)
-    (*     eapply H2. *)
-    (*     (* cbv [CurveAddAlt.my_field_representation my_field_representation] in *. *) *)
-    (*     repeat (try split); ecancel_assumption. *)
-    (*   } *)
-
-    (*   cbv [pointwise_relation Basics.impl]. *)
-
-    (*   repeat straightline. *)
-
-    (*   split; auto. *)
-    (*   split; [admit| ]. (*What is this trace? Check callees to make sure it is not changed*) *)
-
-    (*   do 11 eexists. *)
-    (*   repeat try split. *)
-    (*   4: { *)
-    (*     (* cbv [CurveAddAlt.my_field_representation my_field_representation] in *. *) *)
-    (*     ecancel_assumption. *)
-    (*   } *)
-    (*   3: { eapply group_prop1 in H20. eapply group_prop2; eauto. } *)
-    (*   2: { *)
-    (*     eapply group_prop1 in H18. rewrite H18. *)
-    (*     destruct (word.unsigned r =? 1) eqn:eq. *)
-    (*     { *)
-    (*       subst x0. subst x1. subst x2. pose proof eq. *)
-    (*       (*Prove this at a higher level*) *)
-    (*       assert (word.unsigned r =? 1 = true -> *)
-    (*               (Px, Py, Pz) = scmul (2 ^ iter) (Px_init0, Py_init0, Pz_init0) -> *)
-    (*               (Outx, Outy, Outz) = scmul (Z.to_nat (n_init mod 2 ^ Z.of_nat iter)) (Px_init0, Py_init0, Pz_init0) ->  *)
-    (*               curve_add (Outx, Outy, Outz) (Px, Py, Pz) = scmul (Z.to_nat (n_init mod 2 ^ Z.of_nat (iter + 1))) (Px_init0, Py_init0, Pz_init0) *)
-    (*       ) by admit. *)
-
-    (*       apply H14; eauto. *)
-    (*     } *)
-
-    (*     subst x0. subst x1. subst x2. *)
-    (*     admit. *)
-    (*   } *)
-
-    (*   admit. *)
-
-
-    (* Admitted. *)
-
-
-(*
-  Lemma compile_ladderstep {tr m l functions}
-        (x1 x2 y1 y2 z1 z2 xout1 yout1 zout1 : F) :
-    let v := @ladderstep_gallina _ _ _ _ _ _ three_b x1 x2 y1 y2 z1 z2 xout1 yout1 zout1 in
-    forall {P} {pred: P v -> predicate} {k: nlet_eq_k P v} {k_impl}
-           Rout
-           X1_ptr X1_var X2_ptr X2_var Y1_ptr Y1_var Y2_ptr Y2_var
-           Z1_ptr Z1_var Z2_ptr Z2_var Xout_ptr Xout_var Yout_ptr Yout_var Zout_ptr Zout_var,
-
-      spec_of_ladderstep functions ->
-
-      (FElem (Some tight_bounds) X1_ptr x1 * FElem (Some tight_bounds) X2_ptr x2 *
-       FElem (Some tight_bounds) Y1_ptr y1 * FElem (Some tight_bounds) Y2_ptr y2 *
-       FElem (Some tight_bounds) Z1_ptr z1 * FElem (Some tight_bounds) Z2_ptr z2 *
-       FElem (Some tight_bounds) Xout_ptr xout1 * 
-       FElem (Some tight_bounds) Yout_ptr yout1 * FElem (Some tight_bounds) Zout_ptr zout1 * Rout)%sep m ->
-
-      map.get l X1_var = Some X1_ptr ->
-      map.get l X2_var = Some X2_ptr ->
-      map.get l Y1_var = Some Y1_ptr ->
-      map.get l Y2_var = Some Y2_ptr ->
-      map.get l Z1_var = Some Z1_ptr ->
-      map.get l Z2_var = Some Z2_ptr ->
-      map.get l Xout_var = Some Xout_ptr ->
-      map.get l Yout_var = Some Yout_ptr ->
-      map.get l Zout_var = Some Zout_ptr ->
-
-      (let v := v in
-       forall (* output values *) m',
-       let '\<Xout', Yout', Zout'\> := @ladderstep_gallina _ _ _ _ _ _ three_b x1 x2 y1 y2 z1 z2 xout1 yout1 zout1 in
-            (FElem (Some tight_bounds) X1_ptr x1 * FElem (Some tight_bounds) X2_ptr x2 *
-            FElem (Some tight_bounds) Y1_ptr y1 * FElem (Some tight_bounds) Y2_ptr y2 *
-            FElem (Some tight_bounds) Z1_ptr z1 * FElem (Some tight_bounds) Z2_ptr z2 *
-            FElem (Some tight_bounds) Xout_ptr Xout' * 
-            FElem (Some tight_bounds) Yout_ptr Yout' * FElem (Some tight_bounds) Zout_ptr Zout' * Rout)%sep m' ->
-         (<{ Trace := tr;
-             Memory := m';
-             Locals := l;
-             Functions := functions }>
-          k_impl
-          <{ pred (k v eq_refl) }>)) ->
-
-      <{ Trace := tr;
-         Memory := m;
-         Locals := l;
-         Functions := functions }>
-      cmd.seq
-        (cmd.call [] "ladderstep"
-                  [ expr.var X1_var; expr.var X2_var;
-                  expr.var Y1_var; expr.var Y2_var;
-                  expr.var Z1_var; expr.var Z2_var;
-                  expr.var Xout_var; expr.var Yout_var;
-                  expr.var Zout_var])
-        k_impl
-      <{ pred (nlet_eq
-                 [Xout_var; Yout_var; Zout_var]
-                 v k) }>.
-  Proof.
-    repeat straightline'.
-    handle_call.
-    apply H10.
-    rewrite H13.
-    ecancel_assumption.
-  Qed.
-
-  Local Ltac ecancel_assumption ::=  repeat rewrite <- Hbounds_eq in *; ecancel_assumption_impl.
-
-  (*Why must these instances be included?*)
-
-  Instance spec_of_mul : spec_of (@mul field_parameters).
-  Proof.
-    pose proof (binop_spec bin_mul). cbv [spec_of]. eapply X.
-  Defined.
-
-  (* Instance spec_of_square : spec_of (@square field_parameters).
-  Proof.
-    pose proof (unop_spec un_square). cbv [spec_of]. eapply X.
-  Defined. *)
-
-  Instance spec_of_add : spec_of (@add field_parameters).
-  Proof.
-    pose proof (binop_spec bin_add). cbv [spec_of]. eapply X.
-  Defined.
-
-  Instance spec_of_sub : spec_of (@sub field_parameters).
-  Proof.
-    pose proof (binop_spec bin_sub). cbv [spec_of]. eapply X.
-  Defined.
-
-  Instance spec_of_from_list : spec_of (@from_list field_parameters).
-  Proof.
-    pose proof (spec_of_from_list (feval three_b)). exact X.
-  Defined.
-
-  (* Instance spec_of_scmula24 : spec_of (@scmula24 prime_field_parameters).
-  Proof.
-    pose proof (unop_spec un_scmula24). cbv [spec_of]. eapply X.
-  Defined. *)
-
-  Lemma relax_bounds_FElem_R : forall R x x_ptr, Lift1Prop.impl1 ((FElem (Some tight_bounds) x_ptr x * R)%sep) ((FElem (Some loose_bounds) x_ptr x * R)%sep).
-  Proof.
-    intros. cbv [Lift1Prop.impl1]. intros.
-    destruct H, H, H, H0.
-    eexists; eexists; split; [eapply H | ]. split; eauto. eapply relax_bounds_FElem. auto.
-  Qed.
-
-  Lemma relax_bounds_binop : forall R x x_ptr y y_ptr, Lift1Prop.impl1 ((FElem (Some tight_bounds) x_ptr x * FElem (Some tight_bounds) y_ptr y * R)%sep) ((FElem (Some loose_bounds) x_ptr x * FElem (Some loose_bounds) y_ptr y * R)%sep).
-  Proof.
-    intros. cbv [Lift1Prop.impl1]. intros. eapply sep_assoc. eapply relax_bounds_FElem_R.
-    eapply sep_comm, sep_assoc. eapply relax_bounds_FElem_R. ecancel_assumption.
-  Qed.
-
-  (*tactics for applying field operations*)
-
-  Ltac find_in_map :=
-    repeat first [ erewrite map.get_put_diff; [| intros contra; discriminate] |
-      eapply map.get_put_same].
-
-  (* Local Hint Extern 8 (WeakestPrecondition.cmd _ _ _ _ _ (_ (nlet_eq _ (_ ^ 2)%F _))) =>
-    let Hsquare := (fresh "Hsquare") in pose proof compile_square as Hsquare;
-    rewrite F.pow_2_r; cbv [ Field.prime_field_parameters] in Hsquare;
-    eapply Hsquare; clear Hsquare; shelve : compiler.
-
-    Local Hint Extern 6 (WeakestPrecondition.cmd _ _ _ _ _ (_ (nlet_eq _ (a24 * _)%F _))) =>
-    let Hscmul := (fresh "Hscmul") in epose proof compile_scmula24 as Hscmul;
-    cbv [Compilation2.field_parameters Field.prime_field_parameters] in *;
-    eapply Hscmul; clear Hscmul; shelve : compiler.
-
-  Local Hint Extern 8 (WeakestPrecondition.cmd _ _ _ _ _ (_ (nlet_eq _ (_ * _)%F _))) =>
-    let Hmul := (fresh "Hmul") in pose proof compile_mul as Hmul;
-    cbv [Compilation2.field_parameters Field.prime_field_parameters] in Hmul;
-    eapply Hmul; [| | | try (eapply relax_bounds_binop; ecancel_assumption) | | |]; clear Hmul; shelve : compiler.
-
-    Local Hint Extern 8 (WeakestPrecondition.cmd _ _ _ _ _ (_ (nlet_eq _ (_ - _)%F _))) =>
-    let Hsub := (fresh "Hsub") in epose proof compile_sub as Hsub;
-    cbv [Compilation2.field_parameters Field.prime_field_parameters] in *;
-    eapply Hsub; clear Hsub; shelve : compiler.
-
-  Local Hint Extern 8 (WeakestPrecondition.cmd _ _ _ _ _ (_ (nlet_eq _ (_ + _)%F _))) =>
-    let Hadd := (fresh "Hadd") in epose proof compile_add as Hadd;
-    cbv [Compilation2.field_parameters Field.prime_field_parameters] in *;
-    eapply Hadd; clear Hadd; shelve : compiler.
-
-  Local Hint Extern 9 ((FElem (Some loose_bounds) _ _ ⋆ FElem (Some loose_bounds) _ _ ⋆ _)%sep _) =>
-    eapply relax_bounds_binop; ecancel_assumption : compiler.
-
-  Local Hint Extern 9 =>
-  simple eapply (@compile_stack _ _ _ _ _ _ _ _ _ _ _ _ _ _ _ _ _ _ _ _ _ _
-    ((@FElem width BW word mem prime_field_parameters field_representaton
-    (@None (@bounds field_parameters width BW word mem field_representaton)))));
-    [ecancel_assumption | shelve] : compiler. *)
-
-
-  Lemma FElem_bounds_None : forall x x_ptr R, Lift1Prop.impl1 (FElem (Some loose_bounds) x_ptr x * R)%sep (FElem None x_ptr x * R)%sep.
-  Proof.
-    intros. cbv [Lift1Prop.impl1]; intros m Hsep.
-    destruct Hsep as [m1 [m2 [Hsep1 [Hsep2 Hsep3]]]].
-    do 2 eexists. split; eauto. split; eauto.
-    cbv [FElem Lift1Prop.ex1] in *. sepsimpl. simpl.
-    exists x0. sepsimpl; auto.
-  Qed.
-
-  Local Hint Extern 9 ((FElem None _ _ ⋆ _ )%sep _) =>
-  eapply FElem_bounds_None; ecancel_assumption : compiler_cleanup_post.
-
-  Ltac clear_pred_seps' :=   
-  unfold pred_sep;
-  repeat change (fun x => ?h x) with h;
-  repeat match goal with
-         | [ H : _ ?m |- _ ?m] =>
-           eapply Proper_sep_impl1;
-           [ eapply P_to_bytes | clear H m; intros H m |
-            try (eapply FElem_bounds_None; ecancel_assumption);
-            try (eapply FElem_bounds_None; eapply relax_bounds_FElem_R; ecancel_assumption)]
-         end.
-
-  Hint Extern 1 (pred_sep _ _ _ _ _ _) =>
-         clear_pred_seps'; shelve : compiler_cleanup_post.
-
-  Hint Extern 1 (Some tight_bounds) =>
-         rewrite <- Hbounds_eq : compiler.
-
-  Derive ladderstep_body SuchThat
-         (defn! "ladderstep" ("X1", "X2", "Y1", "Y2", "Z1", "Z2", "Xout", "Yout", "Zout")
-              { ladderstep_body },
-           implements @ladderstep_gallina _ _ _ _ _ _ three_b
-                      using [@mul field_parameters;@add field_parameters;@sub field_parameters; @from_list field_parameters])
-         As ladderstep_correct.
-  Proof.
-    assert (1 + 1 = 2) by lia. 
-    compile_setup.
-    compile_step.
-    compile_step.
-
-    epose proof compile_from_list.
-    eapply H7.
-    5: {
+      repeat straightline'.
+      straightline_call.
       ecancel_assumption.
-    }
-    4: {
-       eapply map.get_put_same.
-    }
-    2: {
-      repeat compile_step.
-    }
-    1: {
-      (*What is this goal??*)
-      compile_step. repeat compile_step.
-    }
-    1: auto.
+      clear dependent mem0.
+
+      repeat straightline'.
+
+      straightline_call.
+      ecancel_assumption.
+      clear dependent a0.
+
+      repeat straightline'.
+
+      straightline_call.
+      sepsimpl.
+      ecancel_assumption.
+      ecancel_assumption.
+      ecancel_assumption.
+      ecancel_assumption.
+
+      cbv [ZRange.is_bounded_by_bool]. simpl.
+      {
+        rewrite <- H10; lia.
+      }
+
+      repeat straightline'.
+      clear dependent a2.
+
+      straightline_call.
+      sepsimpl.
+      ecancel_assumption.
+      ecancel_assumption.
+      ecancel_assumption.
+      clear dependent a0.
+
+      repeat straightline'.
+      straightline_call.
+      sepsimpl.
+      ecancel_assumption.
+      ecancel_assumption.
+      ecancel_assumption.
+      clear dependent a2.
+
+      repeat straightline'.
+
+      rewrite <- H9.
+      rewrite Nat2Z.inj_add.
+      rewrite <- Z.shiftr_shiftr.
+      rewrite Z.shiftr_div_pow2.
+      rewrite Z.pow_1_r.
+      f_equal.
+
+      assumption.
+      lia. lia.
 
 
-    compile_step.
-    compile_step.
-    compile_step.
-    compile_step; compile_step.
-    compile_step.
-    compile_step.
-    compile_step; compile_step.
-    compile_step.
-    compile_step.
-    compile_step; compile_step.
-    compile_step.
-    compile_step.
-    compile_step.
-    compile_step; compile_step.
-    compile_step.
-    compile_step.
-    compile_step; compile_step.
-    compile_step.
-    compile_step.
-    compile_step; compile_step.
-    compile_step.
-    compile_step.
-    compile_step; compile_step.
-    compile_step; compile_step.
-    compile_step; compile_step.
-    compile_step; compile_step.
-    compile_step; compile_step.
-    compile_step.
-    compile_step.
-    compile_step; compile_step.
-    compile_step; compile_step.
-    compile_step; compile_step.
-    compile_step; compile_step.
-    compile_step; compile_step.
-    compile_step; compile_step.
-    compile_step; compile_step.
-    compile_step; compile_step.
-    compile_step; compile_step.
-    compile_step; compile_step.
-    compile_step; compile_step.
-    compile_step; compile_step.
-    compile_step; compile_step.
-    compile_step.
-    compile_step.
-    compile_step; compile_step.
-    compile_step; compile_step.
-    compile_step; compile_step.
-    compile_step; compile_step.
-    compile_step; compile_step.
-    compile_step; compile_step.
-    compile_step; compile_step.
-    compile_step; compile_step.
-    compile_step; compile_step.
-    compile_step; compile_step.
-    compile_step; compile_step.
-    compile_step; compile_step.
-    compile_step; compile_step.
-    compile_step; compile_step.
-    compile_step; compile_step.
-    compile_step; compile_step.
-    compile_step; compile_step.
-    compile_step; compile_step.
-    compile_step; compile_step.
-    compile_step; compile_step.
-    compile_step; compile_step.
-    compile_step; compile_step.
-    compile_step; compile_step.
-    compile_step; compile_step.
-    compile_step; compile_step.
-    compile_step; compile_step.
-    compile_step; compile_step.
-    compile_step; compile_step.
-    compile_step; compile_step.
-  Qed. *)
+      3: ecancel_assumption.
+
+      1: {
+        rewrite Modulo.Z.mod_pow_r_split with (e1:=Z.of_nat iter) by lia.
+        destruct (word.unsigned x =? 1) eqn:E.
+        - subst.
+          rewrite Z2Nat.inj_add.
+          rewrite scmul_add.
+          (* rewrite !Z.pow_1_r. *)
+          rewrite Nat2Z.inj_add.
+          rewrite Z.add_simpl_l.
+          rewrite !Z.pow_1_r.
+          rewrite Z.shiftr_div_pow2 in *.
+          rewrite H5 in *.
+
+          rewrite H10.
+          assert (word.unsigned x = 1) by lia.
+          rewrite H4.
+          rewrite Z.mul_1_r.
+          rewrite <- !H6.
+          rewrite Z2Nat.inj_pow.
+          rewrite Nat2Z.id.
+          replace (Z.to_nat 2) with (2%nat) by reflexivity.
+          rewrite <- H7.
+          apply curve_add_spec.
+          assumption.
+          all: lia.
+        -
+          rewrite Z2Nat.inj_add.
+          rewrite scmul_add.
+          (* rewrite !Z.pow_1_r. *)
+          rewrite Nat2Z.inj_add.
+          rewrite Z.add_simpl_l.
+          rewrite !Z.pow_1_r.
+          rewrite Z.shiftr_div_pow2 in *.
+          rewrite H5 in *.
+
+          rewrite H10.
+          assert (word.unsigned x = 0) by lia.
+          rewrite H4.
+          rewrite Z.mul_0_r.
+          rewrite <- !H6.
+          replace (Z.to_nat 0) with (0%nat) by reflexivity.
+          simpl.
+          apply curve_add_spec.
+          subst x1 x2 x3.
+          assumption.
+          all: lia.
+      }
+
+      rewrite Nat.pow_add_r.
+      simpl.
+      replace (2 ^ iter * 2)%nat with (2 ^ iter + 2 ^ iter)%nat by lia.
+      rewrite scmul_add.
+      rewrite <- H7.
+      apply curve_add_spec. assumption.
+    Qed.
 
 End __.
 (* 
