src/Bedrock/Group/CurveAdd/ScalarMult.v
@@ -1,6 +1,7 @@
-Require Import Rupicola.Lib.Api. Import bedrock2.WeakestPrecondition.
+Require Import Rupicola.Lib.Api.
+Import bedrock2.WeakestPrecondition.
 Require Import Crypto.Arithmetic.PrimeFieldTheorems.
-Require Import Crypto.Bedrock.Group.CurveAdd.StoreZeroGSpec.
+Require Import Crypto.Bedrock.Group.CurveAdd.StoreZero.
 Require Import Crypto.Bedrock.Group.CurveAdd.LoopBody.
 Require Import Crypto.Bedrock.Specs.Field.
 Require Import Crypto.Bedrock.Field.Interface.CompilationAbstract.
@@ -12,10 +13,9 @@ Require Import Crypto.Arithmetic.Core.
 Require Import Crypto.Arithmetic.UniformWeight.
 Local Open Scope Z_scope.
 
-
 Section __.
-  Definition width := 64%Z.
-  Context {BW: Bitwidth width} {word: word.word width} {mem: map.map word Byte.byte}.
+  (* Definition width := 64%Z. *)
+  Context {width : Z} {BW: Bitwidth width} {word: word.word width} {mem: map.map word Byte.byte}.
   Context {locals: map.map String.string word}.
   Context {env: map.map String.string (list String.string * list String.string * Syntax.cmd)}.
   Context {ext_spec: bedrock2.Semantics.ExtSpec}.
@@ -34,63 +34,162 @@ Section __.
   Context {curve_add : (F * F * F) -> (F * F * F) -> (F * F * F)}.
   Context {group_prop1 : forall x y z, curve_add (x, y, z) (Fzero, Fone, Fzero) = (x, y, z)}.
 
-    Instance spec_of_loop_body : spec_of "loop_body" := spec_of_loop_body (curve_add:=curve_add).
+    (* Instance spec_of_loop_body : spec_of "loop_body" := spec_of_loop_body (curve_add:=curve_add). *)
 
-    Instance spec_of_store_zero : spec_of "store_zero_G" := spec_of_store_zero.
+    Instance spec_of_store_zero : spec_of "store_zero" := spec_of_store_zero.
+
+    Context {scalar_words : nat}.
+
+    Definition scalar_bits := (width * Z.of_nat scalar_words).
+
+    Context {scalar_words_ok1 : scalar_bits < 2 ^ width}.
+    (* Context {scalar_words_ok2 : (0 < scalar_words)%nat}. *)
 
     Instance spec_of_scalar_mult : spec_of "scalar_mult" :=
-    fnspec! "scalar_mult"
-          (pPx pPy pPz pOutx pOuty pOutz pn : word)
-          / (Px Py Pz Outx Outy Outz : F) (n : list word) R,
-    { requires tr mem :=
-        (FElem (Some tight_bounds) pPx Px
-         * FElem (Some tight_bounds) pPy Py
-         * FElem (Some tight_bounds) pPz Pz
-         * FElem (Some tight_bounds) pOutx Outx
-         * FElem (Some tight_bounds) pOuty Outy
-         * FElem (Some tight_bounds) pOutz Outz
-         * Bignum.Bignum 6 pn n
-         * R)%sep mem
-         ;
-      ensures tr' mem' :=
-        tr = tr'
-        /\ exists Pxnew Pynew Pznew Outxnew Outynew Outznew (* output values *)
-                  : F,
-           exists nnew : list word,
-               (Outxnew, Outynew, Outznew) = (@scmul _ field_parameters curve_add) (Z.to_nat (Positional.eval (uweight 64) 6 (List.map word.unsigned n))) (Px, Py, Pz)
+      fnspec! "scalar_mult"
+        (pPx pPy pPz pOutx pOuty pOutz pn : word)
+        / (Px Py Pz Outx Outy Outz : F) (n : list word) R,
+        { requires tr mem :=
+            (FElem (Some tight_bounds) pPx Px
+             * FElem (Some tight_bounds) pPy Py
+             * FElem (Some tight_bounds) pPz Pz
+             * FElem (Some tight_bounds) pOutx Outx
+             * FElem (Some tight_bounds) pOuty Outy
+             * FElem (Some tight_bounds) pOutz Outz
+             * Bignum.Bignum scalar_words pn n
+             * R)%sep mem
+        ;
+          ensures tr' mem' :=
+            tr = tr'
+            /\ exists Pxnew Pynew Pznew Outxnew Outynew Outznew (* output values *)
+              : F,
+            exists nnew : list word,
+              (Outxnew, Outynew, Outznew) = (@scmul _ field_parameters curve_add) (Z.to_nat (Positional.eval (uweight width) scalar_words (List.map word.unsigned n))) (Px, Py, Pz)
               /\ (FElem (Some tight_bounds) pPx Pxnew
-                * FElem (Some tight_bounds) pPy Pynew
-                * FElem (Some tight_bounds) pPz Pznew
-                * FElem (Some tight_bounds) pOutx Outxnew
-                * FElem (Some tight_bounds) pOuty Outynew
-                * FElem (Some tight_bounds) pOutz Outznew
-                * Bignum.Bignum 6 pn nnew
-                * R)%sep mem'}.
+                 * FElem (Some tight_bounds) pPy Pynew
+                 * FElem (Some tight_bounds) pPz Pznew
+                 * FElem (Some tight_bounds) pOutx Outxnew
+                 * FElem (Some tight_bounds) pOuty Outynew
+                 * FElem (Some tight_bounds) pOutz Outznew
+                 * Bignum.Bignum scalar_words pn nnew
+                 * R)%sep mem'}.
 
     Require Import bedrock2.NotationsCustomEntry.
     Require Import bedrock2.WeakestPrecondition.
     Import Syntax BinInt String List.ListNotations.
     Local Open Scope string_scope. Local Open Scope Z_scope. Local Open Scope list_scope.
-    
 
+    (* MaxBounds lemmas *)
+    Lemma max_bounds_map_max_range w n : @MaxBounds.max_bounds w n = List.map Some (List.repeat (@MaxBounds.max_range w) n).
+    Proof. rewrite ListUtil.map_repeat. reflexivity. Qed.
+
+    Lemma eval_max_range_lower w n :
+      (0 <= w) ->
+      Positional.eval (uweight w) n (List.map ZRange.lower (List.repeat (@MaxBounds.max_range w) n)) = 0.
+    Proof.
+      intros.
+      induction n.
+      - reflexivity.
+      - simpl.
+        rewrite Positional.eval_cons.
+        rewrite uweight_eval_shift.
+        3, 4: now rewrite map_length, repeat_length.
+        2: assumption.
+        rewrite uweight_0, IHn.
+        lia.
+    Qed.
+
+    Lemma eval_max_range_upper w n :
+      0 <= w ->
+       Positional.eval (uweight w) n (List.map ZRange.upper (List.repeat (@MaxBounds.max_range w) n)) = 2 ^ (w * Z.of_nat n) - 1.
+    Proof.
+      induction n; intros.
+      - simpl.
+        rewrite Z.mul_0_r.
+        rewrite Positional.eval_nil.
+        reflexivity.
+      -
+        rewrite Nat2Z.inj_succ.
+        remember (Z.of_nat n). simpl.
+        rewrite Positional.eval_cons.
+        rewrite uweight_eval_shift.
+        3, 4: now rewrite map_length, repeat_length.
+        2: auto.
+        rewrite uweight_1, uweight_0, IHn; auto.
+        rewrite Z.mul_succ_r.
+        rewrite Z.pow_add_r.
+        nia.
+        nia.
+        nia.
+    Qed.
 
     Ltac solve_locals5 l3 l2 l1 l0 l :=
       subst l3 l2 l1 l0 l; repeat (erewrite map.get_put_diff; [| intros contra; discriminate]); eapply map.get_put_same.
 
-                
-    
+    Ltac update_mem :=
+      match goal with
+      | Hsplit : map.split ?comb ?mem ?stack |- _ =>
+          match goal with
+          | Hold_mem : ?p mem,
+              Hstack : Memory.anybytes ?a felem_size_in_bytes stack
+            |- _ =>
+              let x := fresh "x" in
+              let Hmem := fresh "Hmem" in
+              eapply FElem_from_bytes in Hstack as [x Hstack]
+              ; eassert (Hnew_mem : (p ⋆ FElem None a x) comb) by (eexists; eauto)
+              ; clear dependent mem
+              ; clear dependent stack
+              ; rename Hnew_mem into Hmem
+          | Hold_mem : ?p mem,
+              Hstack : Memory.anybytes ?a (Memory.bytes_per_word _) stack
+            |- _ =>
+              let x := fresh "x" in
+              let Hmem := fresh "Hmem" in
+              eapply anybytes_to_scalar in Hstack as [x Hstack]
+              ; eassert (Hnew_mem : (p ⋆ scalar a x) comb) by (eexists; eauto)
+              ; clear dependent mem
+              ; clear dependent stack
+              ; rename Hnew_mem into Hmem
+          end
+      end.
+
+  Ltac straightline' :=
+    match goal with
+    | |- felem_size_in_bytes mod _ = 0 => eapply felem_size_in_bytes_mod
+    | |- ?a mod ?a = 0 => eapply Z_mod_same_full
+    | _ => update_mem
+    | _ => straightline
+    | l := _ : map.rep |- _ => subst l
+    | l := _ : list word.rep |- _ => subst l
+    | |- Some _ = Some _ => try reflexivity
+    | |- exists _, _ => eexists
+    | |- _ /\ _ => split
+    | |- map.get _ _ = _ => repeat (erewrite map.get_put_diff; [| intros contra; discriminate]); eapply map.get_put_same
+    end.
+
+  Ltac sep_and_fwd :=
+    match goal with
+    | H : context[fun m => _] |- _ =>
+        let Hnew1 := fresh "Hmem" in
+        let Hnew2 := fresh "Hmem" in
+        eassert (Hnew1 : ((fun m => _) ⋆ _) _) by ecancel_assumption;
+        eapply sep_and_l_fwd in Hnew1 as [Hnew1 Hnew2];
+        clear H
+    end.
+
     Definition scalar_mult_func : bedrock2.Syntax.func :=
         ("scalar_mult", (["px"; "py"; "pz"; "outx"; "outy"; "outz"; "pn"], []:list String.string, bedrock_func_body:(
-        stackalloc 48 as pauxx;
-        stackalloc 48 as pauxy;
-        stackalloc 48 as pauxz;
-        stackalloc 8 as cond;
-        stackalloc 8 as iter;
-        coq:(cmd.call [] "store_zero_G" [expr.var "outx"; expr.var "outy"; expr.var "outz"]);
+        stackalloc felem_size_in_bytes as pauxx;
+        stackalloc felem_size_in_bytes as pauxy;
+        stackalloc felem_size_in_bytes as pauxz;
+        stackalloc (Memory.bytes_per_word width) as cond;
+        stackalloc (Memory.bytes_per_word width) as iter;
+        coq:(cmd.call [] "store_zero" [expr.var "outx"; expr.var "outy"; expr.var "outz"]);
         coq:(cmd.store access_size.word (expr.var "iter") (expr.literal 0));
-        while (coq:( expr.op bopname.ltu (expr.load access_size.word (expr.var "iter")) (expr.literal 384) )){
+        while (coq:( expr.op bopname.ltu (expr.load access_size.word (expr.var "iter")) scalar_bits )){
             coq:(cmd.store access_size.word (expr.var "iter") (expr.op bopname.add (expr.load access_size.word "iter") (expr.literal 1)));
-            coq:(cmd.call [] "loop_body" [expr.var "px"; expr.var "py"; expr.var "pz"; expr.var "outx"; expr.var "outy"; expr.var "outz"; expr.var "pauxx"; expr.var "pauxy"; expr.var "pauxz"; expr.var "pn"; expr.var "cond" ])
+            coq:(cmd.call [] "loop_body"
+                   [expr.var "px"; expr.var "py"; expr.var "pz"; expr.var "outx"; expr.var "outy"; expr.var "outz"; expr.var "pauxx"; expr.var "pauxy"; expr.var "pauxz"; expr.var "pn"; expr.var "cond" ])
         }
         ))).
 
@@ -98,78 +197,134 @@ Section __.
         (* Definition c_mod := (c_module (scalar_mult_func :: nil)). *)
         (* Eval native_compute in c_mod. *)
 
+
+    (* Opaque felem_size_in_words. *)
+    Opaque felem_size_in_bytes.
+    Opaque scalar_words.
+    Opaque scalar_bits.
+    Opaque Memory.bytes_per_word.
+    Opaque Z.of_nat.
+
+    (* Lemma width_in_bytes_mod_width : *)
+    (*   width_in_bytes mod Memory.bytes_per_word width = 0. *)
+    (* Proof. *)
+    (*   unfold Memory.bytes_per_word. *)
+
+Require Import Crypto.COperationSpecifications.
+
+    Lemma max_bounds_words : forall (x : list word) n, length x = n -> list_Z_bounded_by (@MaxBounds.max_bounds width n) (List.map word.unsigned x).
+    Proof.
+        intros. generalize dependent x.
+        induction n; intros.
+            - destruct x; try discriminate. simpl. cbv. auto.
+            - destruct x; try discriminate. simpl.
+              eapply Util.list_Z_bounded_by_cons. split.
+              2: {
+                  simpl in IHn. eapply IHn. auto.
+              }
+              apply Expr.is_bounded_by_bool_width_range.
+              eauto.
+              pose proof Properties.word.unsigned_range. auto.
+    Qed.
+
+  Instance spec_of_loop_body : spec_of "loop_body" :=
+    fnspec! "loop_body"
+          (pPx pPy pPz pOutx pOuty pOutz pPauxx pPauxy pPauxz pn pc : word)
+          / (Px Py Pz Outx Outy Outz Pauxx Pauxy Pauxz Px_init Py_init Pz_init : F) (iter : nat) (n_init : Z) (n : list word) (c : word) R,
+    { requires tr mem :=
+        (FElem (Some tight_bounds) pPx Px
+         * FElem (Some tight_bounds) pPy Py
+         * FElem (Some tight_bounds) pPz Pz
+         * FElem (Some tight_bounds) pOutx Outx
+         * FElem (Some tight_bounds) pOuty Outy
+         * FElem (Some tight_bounds) pOutz Outz
+         * FElem None pPauxx Pauxx
+         * FElem None pPauxy Pauxy
+         * FElem None pPauxz Pauxz
+         * Bignum.Bignum scalar_words pn n
+         * scalar pc c
+         * R)%sep mem
+        (* these bounds should be incorporated in the Bignum.Bignum predicate, as it is in FElem *)
+         /\ (Positional.eval (uweight width) scalar_words (List.map word.unsigned n)) = Z.shiftr n_init (Z.of_nat iter)
+         /\ (Outx, Outy, Outz) = scmul (curve_add:=curve_add) (Z.to_nat (n_init mod (2 ^ (Z.of_nat iter))))%Z (Px_init, Py_init, Pz_init)
+         /\ (Px, Py, Pz) = scmul (curve_add:=curve_add) (2 ^ iter) (Px_init, Py_init, Pz_init)
+         ;
+      ensures tr' mem' :=
+        tr = tr'
+        /\ exists Pxnew Pynew Pznew Outxnew Outynew Outznew Pauxxnew Pauxynew Pauxznew (* output values *)
+                  : F,
+           exists nnew : list word,
+           exists cnew : word,
+               (*n*)
+            (Positional.eval (uweight width) scalar_words (List.map word.unsigned nnew)) = Z.shiftr n_init (Z.of_nat (iter + 1))
+            /\ (Outxnew, Outynew, Outznew) = scmul (curve_add:=curve_add) (Z.to_nat (n_init mod (2 ^ (Z.of_nat (iter + 1)))))%Z (Px_init, Py_init, Pz_init)
+            /\ (Pxnew, Pynew, Pznew) = scmul (curve_add:=curve_add) (2 ^ (iter + 1)) (Px_init, Py_init, Pz_init)
+          /\ (FElem (Some tight_bounds) pPx Pxnew
+                * FElem (Some tight_bounds) pPy Pynew
+                * FElem (Some tight_bounds) pPz Pznew
+                * FElem (Some tight_bounds) pOutx Outxnew
+                * FElem (Some tight_bounds) pOuty Outynew
+                * FElem (Some tight_bounds) pOutz Outznew
+                * FElem (Some tight_bounds) pPauxx Pauxxnew
+                * FElem (Some tight_bounds) pPauxy Pauxynew
+                * FElem (Some tight_bounds) pPauxz Pauxznew
+                * Bignum.Bignum scalar_words pn nnew
+                * scalar pc cnew
+                * R)%sep mem'}.
+
     Lemma scalar_mult_ok : program_logic_goal_for_function! scalar_mult_func.
     Proof.
-      cbv [width] in *.
-      cbv [program_logic_goal_for spec_of_scalar_mult]; repeat straightline.
-      cbv [scalar_mult_func].
-      repeat straightline.
-      simpl.
+      enter scalar_mult_func.
+      repeat straightline'.
 
-      eexists; split; [ repeat straightline; cbv [map.of_list_zip]; simpl; eauto |].
-      repeat straightline.
+      eexists; split.
+      cbv [map.of_list_zip]; simpl; eauto.
 
-      eexists; split; [ repeat (repeat straightline; eexists; split; [solve_locals5 l3 l2 l1 l0 l| ]); repeat straightline| ].
+      repeat straightline'.
 
-      pose proof H as Hspec1.
-      cbv [spec_of_store_zero LoopBody.spec_of_store_zero spec_of_store_zero] in Hspec1.
+      straightline_call.
 
+      ecancel_assumption_impl.
+      clear dependent mCombined.
+      repeat straightline'.
 
-      eapply Proper_call; [| eapply Hspec1; ecancel_assumption].
-      cbv [pointwise_relation Basics.impl]. repeat straightline.
-      eexists. split; [subst a6; eauto |].
+      remember #{ "px" => pPx; "py" => pPy; "pz" => pPz; "outx" => pOutx; "outy" => pOuty; "outz" => pOutz; "pn" => pn; "pauxx" => a; "pauxy" => a0; "pauxz" => a1; "cond" => a2; "iter" => a3 }# as l.
 
-      repeat straightline.
-      eexists; split; [repeat straightline; eexists; split; [solve_locals5 l3 l2 l1 l0 l| repeat straightline]| ].
-      eexists; split; [repeat straightline| ].
+      clear dependent a5.
 
-      clear H1 H20 H18 H16 H14 H12.
-      assert (Hwa3 : exists wa3, (scalar a3 wa3) = (array ptsto (word.of_Z 1) a3 stack3)) by admit.
-      assert (Hwa2 : exists wa2, (scalar a2 wa2) = (array ptsto (word.of_Z 1) a2 stack2)) by admit.
+      exists nat.
+      eexists (fun a => (fun b => b < a <= Z.to_nat scalar_bits)%nat).
 
-      destruct Hwa3, Hwa2.
-      rewrite <- H12 in H23.
-      rewrite <- H1 in H23. 
-      (* assert (exists wa3, (scalar a3 wa3) = (array ptsto (word.of_Z 1) a3 stack3)) by admit.
-      assert (exists wa3, (scalar a3 wa3) = (array ptsto (word.of_Z 1) a3 stack3)) by admit.
-      assert (exists wa3, (scalar a3 wa3) = (array ptsto (word.of_Z 1) a3 stack3)) by admit. *)
+      rename a3 into piter.
+      rename v into iter.
 
-      eapply store_word_of_sep; [ecancel_assumption| repeat straightline].
-
-      assert (Hc: exists wc, (scalar a2 x0) = Bignum.Bignum 1 a2 [wc]) by admit.
-      destruct Hc. rewrite H16 in H14; clear H16.
-
-      assert (Hf1 : exists f1, (FElem (Some tight_bounds) a1 f1) = (array ptsto (word.of_Z 1) a1 stack1)) by admit.
-      destruct Hf1. rewrite <- H16 in H14.
-
-      assert (Hf0 : exists f0, (FElem (Some tight_bounds) a0 f0) = (array ptsto (word.of_Z 1) a0 stack0)) by admit.
-      destruct Hf0. rewrite <- H18 in H14.
-
-      assert (Hf : exists f, (FElem (Some tight_bounds) a f) = (array ptsto (word.of_Z 1) a stack)) by admit.
-      destruct Hf. rewrite <- H20 in H14.
-
-      clear H16 H18 H20.
+      rename a2 into pc.
+      rename x2 into c.
 
       rename a into pPauxx.
       rename a0 into pPauxy.
       rename a1 into pPauxz.
-      rename a2 into pc.
-      rename a3 into piter.
+      rename x into pauxx.
+      rename x0 into pauxy.
+      rename x1 into pauxz.
 
+      remember ((Positional.eval (uweight width) scalar_words (List.map word.unsigned n))) as n_init.
 
-      remember ((Positional.eval (uweight 64) 6 (List.map word.unsigned n))) as n_init.
-      remember (Px) as Px_init.
-      remember (Py) as Py_init.
-      remember (Pz) as Pz_init.
+      assert (nlength : Datatypes.length n = scalar_words).
+      { eassert (htemp : (Bignum.Bignum _ _ _ ⋆ _) _) by ecancel_assumption.
+        destruct htemp as [?[?[?[htemp ?]]]].
+        destruct htemp as [?[?[?[htemp ?]]]].
+      destruct htemp. assumption. }
 
+      rename Px into Px_old.
+      rename Py into Py_old.
+      rename Pz into Pz_old.
 
-      eexists nat. eexists (fun s => (fun b => b < s < 400)%nat).
+      rename a4 into tr.
 
-
-      (*Invariant*)
-      
-      exists ( fun (v : nat) (tr : Semantics.trace) (m' : mem) (l' : locals) =>
-        l' = l3 /\
+      exists ( fun (v : nat) (tr' : Semantics.trace) (m' : mem) (l' : locals) =>
+        l' = l /\
+        tr' = tr /\
           exists Pauxx Pauxy Pauxz c viter Px Py Pz Outx Outy Outz n,
 
         ( scalar piter (word.of_Z viter)
@@ -179,189 +334,477 @@ Section __.
         * FElem (Some tight_bounds) pOutx Outx
         * FElem (Some tight_bounds) pOuty Outy
         * FElem (Some tight_bounds) pOutz Outz
-        * FElem (Some tight_bounds) pPauxx Pauxx
-        * FElem (Some tight_bounds) pPauxy Pauxy
-        * FElem (Some tight_bounds) pPauxz Pauxz
-        * Bignum.Bignum 6 pn n
-        * Bignum.Bignum 1 pc [c]
+        * FElem None pPauxx Pauxx
+        * FElem None pPauxy Pauxy
+        * FElem None pPauxz Pauxz
+        * Bignum.Bignum scalar_words pn n
+        * scalar pc c
         * R)%sep m'
-        /\ (*n*)
-           (Positional.eval (uweight 64) 6 (List.map word.unsigned n)) = Z.shiftr n_init (Z.of_nat v)
-        /\ (Outx, Outy, Outz) = @scmul _ field_parameters curve_add  (Z.to_nat (n_init mod (2 ^ (Z.of_nat v))))%Z (Px_init, Py_init, Pz_init)
-        /\ (Px, Py, Pz) = @scmul _ field_parameters curve_add (2 ^ v) (Px_init, Py_init, Pz_init)
-        /\ viter = Z.of_nat (v)
-        /\ viter < 399
+        /\ (Positional.eval (uweight width) scalar_words (List.map word.unsigned n)) = Z.shiftr n_init (Z.of_nat v)
+        /\ (Outx, Outy, Outz) = @scmul _ field_parameters curve_add  (Z.to_nat (n_init mod (2 ^ (Z.of_nat v))))%Z (Px_old, Py_old, Pz_old)
+        /\ (Px, Py, Pz) = @scmul _ field_parameters curve_add (2 ^ v) (Px_old, Py_old, Pz_old)
+        /\ viter = Z.of_nat v
+        /\ (Z.of_nat v <= scalar_bits)
       ).
-
-
       split.
-      {
-        admit.
-      }
-
+      eapply Nat.gt_wf.
       split.
-      {
-        exists 0%nat. split; [reflexivity |]. exists x4. exists x3. exists x2. exists x1. exists 0. exists Px_init, Py_init, Pz_init.
-        exists Fzero, Fone, Fzero. exists n.
-        
-        split; [| split; [| split; [| split]]].
-          - ecancel_assumption.
-          - rewrite Z.shiftr_0_r. subst n_init. eauto.
-          - assert (2 ^ Z.of_nat 0 = 1) by admit.
-            assert (n_init mod 1 = 0) by admit.
-            rewrite H16, H18. simpl. eauto.
-          - simpl. rewrite group_prop1. eauto.
-          - lia.
-      }
+      exists 0%nat.
+      split. auto.
+      split. auto.
+      do 3 eexists.
+      do 9 eexists.
+      split.
+      ecancel_assumption.
+      split.
+      rewrite Z.shiftr_0_r.
+      easy.
+      split.
 
-      repeat straightline.
+      rewrite Z.pow_0_r.
+      rewrite Z.mod_1_r.
+      simpl.
+      reflexivity.
+      simpl.
+      rewrite group_prop1.
+      split; auto.
+      split; auto.
+      Transparent scalar_bits.
+      unfold scalar_bits.
+      destruct word_ok.
+      clear -width_pos.
+      nia.
+
+      intros.
+
       eexists; split.
-      {
-        (repeat straightline; eexists; split; [solve_locals5 l3 l2 l1 l0 l| repeat straightline]).
-        eexists. split.
-          - repeat straightline.
-            eapply load_word_of_sep. ecancel_assumption.
-          - repeat straightline.
-      }
+      cbv [map.of_list_zip]; simpl; eauto.
+
+      repeat straightline'.
+      clear dependent m.
+
+      destruct H2.
+      destruct H2.
+      rewrite H2.
+
+      split.
+      repeat straightline'.
+      clear dependent m0.
+
+      straightline_call.
+      split.
+      ecancel_assumption.
+
+      split.
+      (* admit. *)
+      (* split. *)
+
+
+      eassumption.
+      split.
+      eassumption.
+      eassumption.
+      clear dependent m.
+
+      repeat straightline'.
+
+      rewrite <- word.ring_morph_add in H11.
+      subst x4.
+      replace (Z.of_nat v + 1) with (Z.of_nat (v + 1)) in H11 by lia.
+
+      (* clear H4 H5 H6. *)
+
+      ecancel_assumption_impl.
+      eassumption.
+      eassumption.
+      eassumption.
+
+      destruct (word.ltu (word.of_Z (Z.of_nat v)) (word.of_Z scalar_bits)) eqn:E.
+      rewrite <- word.morph_ltu in E.
+      lia.
+      lia.
+      lia.
+      rewrite word.unsigned_of_Z_0 in H4. lia.
+      lia.
+      destruct (word.ltu (word.of_Z (Z.of_nat v)) (word.of_Z scalar_bits)) eqn:E.
+      rewrite <- word.morph_ltu in E.
+      lia.
+      lia.
+      lia.
+      rewrite word.unsigned_of_Z_0 in H4. lia.
 
       repeat straightline.
-      split.
-      {
-        repeat straightline.
-        eexists; split.
-        {
-          (repeat straightline; eexists; split; [solve_locals5 l3 l2 l1 l0 l| repeat straightline]).
-        }
 
-        repeat straightline.
-        eexists; split.
-        {
-          (repeat straightline; eexists; split; [solve_locals5 l3 l2 l1 l0 l| repeat straightline]).
-          eexists; split; repeat straightline.
-          eapply load_word_of_sep. ecancel_assumption.
-        }
+      (* this is hacky, but note the order has to match order of the exists in the goal *)
+      eassert ((_
+                  ⋆ FElem _ pPauxx _
+                  ⋆ FElem _ pPauxy _
+                  ⋆ FElem _ pPauxz _
+                  ⋆ scalar pc _
+                  ⋆ scalar piter _) m0) by ecancel_assumption.
+      clear H3.
+      (* destruct H2 as [mq'[mr'[hs' [h'' Hr']]]]. *)
+      (* destruct H2 as [?[?[?[? ?]]]]. *)
+      do 5 match goal with
+             | H : (_ ⋆ _) _ |- _ =>
+                 let mq := fresh "mq" in
+                 let mr := fresh "mr" in
+                 let Hs := fresh "Hs" in
+                 let H' := fresh "H" in
+                 let Hr := fresh "Hr" in
+                 destruct H as [mq[mr[Hs [H' Hr]]]]
+             (* | H : FElem _ _ _ _ |- _ => eapply drop_bounds_FElem in H; eapply FElem_from_bytes in H *)
+             (* | H : scalar _ _ _ |- _ => eapply scalar_to_anybytes in H *)
+             end.
+      eexists. eexists. split; [|split].
+      eapply scalar_to_anybytes. eassumption.
+      eassumption.
+      eexists. eexists. split; [|split].
+      eapply scalar_to_anybytes. eassumption.
+      eassumption.
+      eexists. eexists. split; [|split].
+      eapply FElem_from_bytes. eexists. eassumption.
+      eassumption.
+      eexists. eexists. split; [|split].
+      eapply FElem_from_bytes. eexists. eassumption.
+      eassumption.
+      eexists. eexists. split; [|split].
+      eapply FElem_from_bytes. eexists. eassumption.
+      eassumption.
 
-        eapply store_word_of_sep; [ecancel_assumption| ].
+      destruct (word.ltu (word.of_Z (Z.of_nat v)) (word.of_Z scalar_bits)) eqn:E.
+      rewrite word.unsigned_of_Z_1 in H4. discriminate.
+      rewrite <- word.morph_ltu in E.
+      subst x4.
+      assert (Heq : Z.of_nat v = scalar_bits) by lia.
+      rewrite Heq in *.
 
-        repeat straightline.
-        eexists; split.
-        {
-          repeat (repeat straightline; eexists; split; [solve_locals5 l3 l2 l1 l0 l| repeat straightline]).
-        }
+      repeat straightline'.
+      rewrite Z.mod_small in H6.
+      eassumption.
+(* Signature.max_bounds_words *)
+      unshelve epose proof
+        eval_list_Z_bounded_by
+        (uweight width)
+        scalar_words
+        (@MaxBounds.max_bounds width scalar_words)
+        (List.repeat (@MaxBounds.max_range width) scalar_words)
+        (List.map word.unsigned n)
+        _ _ _ _.
+      eapply max_bounds_words.
 
-        eapply Proper_call.
+      eassert ((Bignum.Bignum _ _ _ ⋆ _) _) by ecancel_assumption.
+      destruct H1 as [mq'[mr'[hs[h1 h2]]]].
+      destruct h1 as [mq''[mr''[hs'[h1' h2']]]].
+      destruct h1'.
+      assumption.
+      eapply max_bounds_map_max_range.
+      now rewrite repeat_length.
+      intros.
 
-        2: {
-          pose proof H0 as Hspec2. cbv [spec_of_loop_body LoopBody.spec_of_loop_body] in Hspec2.
+      unshelve epose proof uwprops width _.
+      destruct word_ok.
+      assumption.
+      destruct H3.
+      lia.
 
-          specialize (Hspec2  pPx pPy pPz pOutx pOuty pOutz pPauxx pPauxy pPauxz pn pc).
+      rewrite eval_max_range_lower in H1.
+      rewrite eval_max_range_upper in H1.
+      subst n_init.
+      unfold scalar_bits.
+      lia.
+      destruct word_ok.
+      clear -width_pos.
+      lia.
 
-          eapply Hspec2; clear Hspec2.
-          split; [| split; [| split]].
-
-            - clear H18 H14 H23.  ecancel_assumption.
-            - erewrite <- H20. eauto.
-            - rewrite H22. eauto.
-            - eassumption.
-        }
-
-        cbv [pointwise_relation Basics.impl].
-        repeat straightline.
-        eexists; split; [subst a1; eauto| ].
-
-        eexists. split; [split; eauto | ].
-        1: {
-          do 12 eexists.
-          split; [| split; [| split; [| split; [| split] ]]].
-          1: {
-            rewrite <- word.ring_morph_add in H32.
-            ecancel_assumption.
-          }
-          5: {
-            subst x9. destruct (word.ltu (word.of_Z (Z.of_nat v)) (word.of_Z 384)) eqn:eq.
-              2: {
-                rewrite word.unsigned_of_Z in H16. assert (@word.wrap width word word_ok Z0 = 0) by (cbv [word.wrap width]; lia).
-                rewrite H27 in H16.
-                exfalso. apply H16. auto.
-              }
-              pose proof eq. Search (word.ltu).
-              erewrite <- word.morph_ltu in H27.
-              3: cbv [width]; lia.
-              2: split; cbv [width]; lia.
-              lia.
-              }
-          4: {
-            subst x9.
-            assert (Z.of_nat ((v)) + 1 = Z.of_nat (v + 1)) by lia.
-            eapply H27.
-          }
-          3: eauto.
-          2: eauto.
-          eauto.
-        }
-        split; try lia.
-      }
-      repeat straightline.
-
-      assert (Memory.anybytes piter 8 = scalar piter (word.of_Z x9)) by admit.
-      rewrite H25.
-      eassert ((scalar piter (word.of_Z x9) * _)%sep m0) by ecancel_assumption.
-      destruct H27, H27, H27, H28.
-      eexists. eexists. split.
-      {
-        eapply H28.
-      }
-      split; [apply map.split_comm; eauto| ].
-
-      assert (Memory.anybytes pc 8 = Bignum.Bignum 1 pc [x8]) by admit.
-      rewrite H30.
-      eassert ((Bignum.Bignum 1 pc [x8] * _)%sep x18) by ecancel_assumption.
-      destruct H31, H31, H31, H32.
-      do 2 eexists. split; eauto.
-      split; [eapply map.split_comm; eauto| ].
-
-      assert (Memory.anybytes pPauxz 48 = FElem (Some tight_bounds) pPauxz x7) by admit.
-      rewrite H34.
-      eassert ((FElem (Some tight_bounds) pPauxz x7 * _)%sep x20) by ecancel_assumption.
-      destruct H35, H35, H35, H36.
-      do 2 eexists. split; eauto.
-      split; [eapply map.split_comm; eauto| ].
-
-      assert (Memory.anybytes pPauxy 48 = FElem (Some tight_bounds) pPauxy x6) by admit.
-      rewrite H38.
-      eassert ((FElem (Some tight_bounds) pPauxy x6 * _)%sep x22) by ecancel_assumption.
-      destruct H39, H39, H39, H40.
-      do 2 eexists. split; eauto.
-      split; [eapply map.split_comm; eauto| ].
-
-      assert (Memory.anybytes pPauxx 48 = FElem (Some tight_bounds) pPauxx x5) by admit.
-      rewrite H42.
-      eassert ((FElem (Some tight_bounds) pPauxx x5 * _)%sep x24) by ecancel_assumption.
-      destruct H43, H43, H43, H44.
-      do 2 eexists. split; eauto.
-      split; [eapply map.split_comm; eauto| ].
-      split; eauto.
-      split.
-      1: admit. (*What is this trace even supposed to do????*)
-      do 7 eexists. split.
-      2: {
-        ecancel_assumption.
-      }
-      1: {
-        eauto.
-        rewrite H22.
-        assert (n_init mod 2 ^ (Z.of_nat v) = n_init) by admit.
-        rewrite H46.
-        eauto.
-    Admitted.
-
-    
+      destruct word_ok.
+      clear -width_pos.
+      lia.
 
 
 
-    From bedrock2 Require Import ToCString Bytedump.
-    Definition c_mod := (c_module (scalar_mult_func :: nil)).
 
-    Eval native_compute in c_mod.
+      ecancel_assumption.
+
+      lia.
+      lia.
+      Qed.
+
+     (* match goal with *)
+     (* | Hsplit : map.split ?comb ?mem ?stack |- _ => *)
+     (*     match goal with *)
+     (*       Hold_mem : ?p mem, *)
+     (*         Hstack : Memory.anybytes ?a felem_size_in_bytes stack *)
+     (*       |- _ => *)
+     (*         let x := fresh "x" in *)
+     (*         let Hmem := fresh "Hmem" in *)
+     (*         eapply FElem_from_bytes in Hstack as [x Hstack] *)
+     (*         ; eassert (Hnew_mem : (p ⋆ FElem None a x) comb) by (eexists; eauto) *)
+     (*         ; clear dependent mem *)
+     (*         ; clear dependent stack *)
+     (*         ; rename Hnew_mem into Hmem *)
+     (*     end *)
+     (* end. *)
+     (*  update_mem. *)
+
+     (*  straightline_call. *)
+
+     (*  eexists; split; [ repeat (repeat straightline; eexists; split; [solve_locals5 l3 l2 l1 l0 l| ]); repeat straightline| ]. *)
+
+     (*  straightline_call. *)
+
+     (*  { *)
+     (*    ecancel_assumption_impl. *)
+
+     (*  } *)
+
+     (*  eapply Proper_call; [| eapply Hspec1; ecancel_assumption]. *)
+     (*  cbv [pointwise_relation Basics.impl]. repeat straightline. *)
+     (*  eexists. split; [subst a6; eauto |]. *)
+
+     (*  repeat straightline. *)
+     (*  eexists; split; [repeat straightline; eexists; split; [solve_locals5 l3 l2 l1 l0 l| repeat straightline]| ]. *)
+     (*  eexists; split; [repeat straightline| ]. *)
+
+     (*  clear H1 H20 H18 H16 H14 H12. *)
+     (*  assert (Hwa3 : exists wa3, (scalar a3 wa3) = (array ptsto (word.of_Z 1) a3 stack3)) by admit. *)
+     (*  assert (Hwa2 : exists wa2, (scalar a2 wa2) = (array ptsto (word.of_Z 1) a2 stack2)) by admit. *)
+
+     (*  destruct Hwa3, Hwa2. *)
+     (*  rewrite <- H12 in H23. *)
+     (*  rewrite <- H1 in H23.  *)
+      (* assert (exists wa3, (scalar a3 wa3) = (array ptsto (word.of_Z 1) a3 stack3)) by admit.
+      assert (exists wa3, (scalar a3 wa3) = (array ptsto (word.of_Z 1) a3 stack3)) by admit.
+      assert (exists wa3, (scalar a3 wa3) = (array ptsto (word.of_Z 1) a3 stack3)) by admit. *)
+
+      (* eapply store_word_of_sep; [ecancel_assumption| repeat straightline]. *)
+
+      (* assert (Hc: exists wc, (scalar a2 x0) = Bignum.Bignum 1 a2 [wc]) by admit. *)
+      (* destruct Hc. rewrite H16 in H14; clear H16. *)
+
+      (* assert (Hf1 : exists f1, (FElem (Some tight_bounds) a1 f1) = (array ptsto (word.of_Z 1) a1 stack1)) by admit. *)
+      (* destruct Hf1. rewrite <- H16 in H14. *)
+
+      (* assert (Hf0 : exists f0, (FElem (Some tight_bounds) a0 f0) = (array ptsto (word.of_Z 1) a0 stack0)) by admit. *)
+      (* destruct Hf0. rewrite <- H18 in H14. *)
+
+      (* assert (Hf : exists f, (FElem (Some tight_bounds) a f) = (array ptsto (word.of_Z 1) a stack)) by admit. *)
+      (* destruct Hf. rewrite <- H20 in H14. *)
+
+      (* clear H16 H18 H20. *)
+
+      (* rename a into pPauxx. *)
+      (* rename a0 into pPauxy. *)
+      (* rename a1 into pPauxz. *)
+      (* rename a2 into pc. *)
+      (* rename a3 into piter. *)
+
+
+      (* remember ((Positional.eval (uweight 64) 6 (List.map word.unsigned n))) as n_init. *)
+      (* remember (Px) as Px_init. *)
+      (* remember (Py) as Py_init. *)
+      (* remember (Pz) as Pz_init. *)
+
+
+      (* eexists nat. eexists (fun s => (fun b => b < s < 400)%nat). *)
+
+
+      (*Invariant*)
+      
+    (*   exists ( fun (v : nat) (tr : Semantics.trace) (m' : mem) (l' : locals) => *)
+    (*     l' = l3 /\ *)
+    (*       exists Pauxx Pauxy Pauxz c viter Px Py Pz Outx Outy Outz n, *)
+
+    (*     ( scalar piter (word.of_Z viter) *)
+    (*     * FElem (Some tight_bounds) pPx Px *)
+    (*     * FElem (Some tight_bounds) pPy Py *)
+    (*     * FElem (Some tight_bounds) pPz Pz *)
+    (*     * FElem (Some tight_bounds) pOutx Outx *)
+    (*     * FElem (Some tight_bounds) pOuty Outy *)
+    (*     * FElem (Some tight_bounds) pOutz Outz *)
+    (*     * FElem (Some tight_bounds) pPauxx Pauxx *)
+    (*     * FElem (Some tight_bounds) pPauxy Pauxy *)
+    (*     * FElem (Some tight_bounds) pPauxz Pauxz *)
+    (*     * Bignum.Bignum 6 pn n *)
+    (*     * Bignum.Bignum 1 pc [c] *)
+    (*     * R)%sep m' *)
+    (*     /\ (*n*) *)
+    (*        (Positional.eval (uweight 64) 6 (List.map word.unsigned n)) = Z.shiftr n_init (Z.of_nat v) *)
+    (*     /\ (Outx, Outy, Outz) = @scmul _ field_parameters curve_add  (Z.to_nat (n_init mod (2 ^ (Z.of_nat v))))%Z (Px_init, Py_init, Pz_init) *)
+    (*     /\ (Px, Py, Pz) = @scmul _ field_parameters curve_add (2 ^ v) (Px_init, Py_init, Pz_init) *)
+    (*     /\ viter = Z.of_nat (v) *)
+    (*     /\ viter < 399 *)
+    (*   ). *)
+
+
+    (*   split. *)
+    (*   { *)
+    (*     admit. *)
+    (*   } *)
+
+    (*   split. *)
+    (*   { *)
+    (*     exists 0%nat. split; [reflexivity |]. exists x4. exists x3. exists x2. exists x1. exists 0. exists Px_init, Py_init, Pz_init. *)
+    (*     exists Fzero, Fone, Fzero. exists n. *)
+
+    (*     split; [| split; [| split; [| split]]]. *)
+    (*       - ecancel_assumption. *)
+    (*       - rewrite Z.shiftr_0_r. subst n_init. eauto. *)
+    (*       - assert (2 ^ Z.of_nat 0 = 1) by admit. *)
+    (*         assert (n_init mod 1 = 0) by admit. *)
+    (*         rewrite H16, H18. simpl. eauto. *)
+    (*       - simpl. rewrite group_prop1. eauto. *)
+    (*       - lia. *)
+    (*   } *)
+
+    (*   repeat straightline. *)
+    (*   eexists; split. *)
+    (*   { *)
+    (*     (repeat straightline; eexists; split; [solve_locals5 l3 l2 l1 l0 l| repeat straightline]). *)
+    (*     eexists. split. *)
+    (*       - repeat straightline. *)
+    (*         eapply load_word_of_sep. ecancel_assumption. *)
+    (*       - repeat straightline. *)
+    (*   } *)
+
+    (*   repeat straightline. *)
+    (*   split. *)
+    (*   { *)
+    (*     repeat straightline. *)
+    (*     eexists; split. *)
+    (*     { *)
+    (*       (repeat straightline; eexists; split; [solve_locals5 l3 l2 l1 l0 l| repeat straightline]). *)
+    (*     } *)
+
+    (*     repeat straightline. *)
+    (*     eexists; split. *)
+    (*     { *)
+    (*       (repeat straightline; eexists; split; [solve_locals5 l3 l2 l1 l0 l| repeat straightline]). *)
+    (*       eexists; split; repeat straightline. *)
+    (*       eapply load_word_of_sep. ecancel_assumption. *)
+    (*     } *)
+
+    (*     eapply store_word_of_sep; [ecancel_assumption| ]. *)
+
+    (*     repeat straightline. *)
+    (*     eexists; split. *)
+    (*     { *)
+    (*       repeat (repeat straightline; eexists; split; [solve_locals5 l3 l2 l1 l0 l| repeat straightline]). *)
+    (*     } *)
+
+    (*     eapply Proper_call. *)
+
+    (*     2: { *)
+    (*       pose proof H0 as Hspec2. cbv [spec_of_loop_body LoopBody.spec_of_loop_body] in Hspec2. *)
+
+    (*       specialize (Hspec2  pPx pPy pPz pOutx pOuty pOutz pPauxx pPauxy pPauxz pn pc). *)
+
+    (*       eapply Hspec2; clear Hspec2. *)
+    (*       split; [| split; [| split]]. *)
+
+    (*         - clear H18 H14 H23.  ecancel_assumption. *)
+    (*         - erewrite <- H20. eauto. *)
+    (*         - rewrite H22. eauto. *)
+    (*         - eassumption. *)
+    (*     } *)
+
+    (*     cbv [pointwise_relation Basics.impl]. *)
+    (*     repeat straightline. *)
+    (*     eexists; split; [subst a1; eauto| ]. *)
+
+    (*     eexists. split; [split; eauto | ]. *)
+    (*     1: { *)
+    (*       do 12 eexists. *)
+    (*       split; [| split; [| split; [| split; [| split] ]]]. *)
+    (*       1: { *)
+    (*         rewrite <- word.ring_morph_add in H32. *)
+    (*         ecancel_assumption. *)
+    (*       } *)
+    (*       5: { *)
+    (*         subst x9. destruct (word.ltu (word.of_Z (Z.of_nat v)) (word.of_Z 384)) eqn:eq. *)
+    (*           2: { *)
+    (*             rewrite word.unsigned_of_Z in H16. assert (@word.wrap width word word_ok Z0 = 0) by (cbv [word.wrap width]; lia). *)
+    (*             rewrite H27 in H16. *)
+    (*             exfalso. apply H16. auto. *)
+    (*           } *)
+    (*           pose proof eq. Search (word.ltu). *)
+    (*           erewrite <- word.morph_ltu in H27. *)
+    (*           3: cbv [width]; lia. *)
+    (*           2: split; cbv [width]; lia. *)
+    (*           lia. *)
+    (*           } *)
+    (*       4: { *)
+    (*         subst x9. *)
+    (*         assert (Z.of_nat ((v)) + 1 = Z.of_nat (v + 1)) by lia. *)
+    (*         eapply H27. *)
+    (*       } *)
+    (*       3: eauto. *)
+    (*       2: eauto. *)
+    (*       eauto. *)
+    (*     } *)
+    (*     split; try lia. *)
+    (*   } *)
+    (*   repeat straightline. *)
+
+    (*   assert (Memory.anybytes piter 8 = scalar piter (word.of_Z x9)) by admit. *)
+    (*   rewrite H25. *)
+    (*   eassert ((scalar piter (word.of_Z x9) * _)%sep m0) by ecancel_assumption. *)
+    (*   destruct H27, H27, H27, H28. *)
+    (*   eexists. eexists. split. *)
+    (*   { *)
+    (*     eapply H28. *)
+    (*   } *)
+    (*   split; [apply map.split_comm; eauto| ]. *)
+
+    (*   assert (Memory.anybytes pc 8 = Bignum.Bignum 1 pc [x8]) by admit. *)
+    (*   rewrite H30. *)
+    (*   eassert ((Bignum.Bignum 1 pc [x8] * _)%sep x18) by ecancel_assumption. *)
+    (*   destruct H31, H31, H31, H32. *)
+    (*   do 2 eexists. split; eauto. *)
+    (*   split; [eapply map.split_comm; eauto| ]. *)
+
+    (*   assert (Memory.anybytes pPauxz 48 = FElem (Some tight_bounds) pPauxz x7) by admit. *)
+    (*   rewrite H34. *)
+    (*   eassert ((FElem (Some tight_bounds) pPauxz x7 * _)%sep x20) by ecancel_assumption. *)
+    (*   destruct H35, H35, H35, H36. *)
+    (*   do 2 eexists. split; eauto. *)
+    (*   split; [eapply map.split_comm; eauto| ]. *)
+
+    (*   assert (Memory.anybytes pPauxy 48 = FElem (Some tight_bounds) pPauxy x6) by admit. *)
+    (*   rewrite H38. *)
+    (*   eassert ((FElem (Some tight_bounds) pPauxy x6 * _)%sep x22) by ecancel_assumption. *)
+    (*   destruct H39, H39, H39, H40. *)
+    (*   do 2 eexists. split; eauto. *)
+    (*   split; [eapply map.split_comm; eauto| ]. *)
+
+    (*   assert (Memory.anybytes pPauxx 48 = FElem (Some tight_bounds) pPauxx x5) by admit. *)
+    (*   rewrite H42. *)
+    (*   eassert ((FElem (Some tight_bounds) pPauxx x5 * _)%sep x24) by ecancel_assumption. *)
+    (*   destruct H43, H43, H43, H44. *)
+    (*   do 2 eexists. split; eauto. *)
+    (*   split; [eapply map.split_comm; eauto| ]. *)
+    (*   split; eauto. *)
+    (*   split. *)
+    (*   1: admit. (*What is this trace even supposed to do????*) *)
+    (*   do 7 eexists. split. *)
+    (*   2: { *)
+    (*     ecancel_assumption. *)
+    (*   } *)
+    (*   1: { *)
+    (*     eauto. *)
+    (*     rewrite H22. *)
+    (*     assert (n_init mod 2 ^ (Z.of_nat v) = n_init) by admit. *)
+    (*     rewrite H46. *)
+    (*     eauto. *)
+    (* Admitted. *)
+
+
+
+
+
+    (* From bedrock2 Require Import ToCString Bytedump. *)
+    (* Definition c_mod := (c_module (scalar_mult_func :: nil)). *)
+
+    (* Eval native_compute in c_mod. *)
 
     End __.
