src/Bedrock/Group/CurveAdd/CurveAdd.v
@@ -80,10 +80,11 @@ Section __.
 
   Context (Hbounds_eq : loose_bounds = tight_bounds).
   Context (three_b : felem).
+  Context (three_b_name : string).
   Context (Hb_bounds : maybe_bounded (Some loose_bounds) three_b).
 
-  Instance spec_of_ladderstep : spec_of "ladderstep" :=
-    fnspec! "ladderstep"
+  Instance spec_of_ladderstep : spec_of "curve_add" :=
+    fnspec! "curve_add"
           (pX1 pX2 pY1 pY2 pZ1 pZ2 pXout pYout pZout : word)
           / (X1 X2 Y1 Y2 Z1 Z2 Xoutold Youtold Zoutold : F) R,
     { requires tr mem :=
@@ -158,7 +159,7 @@ Section __.
          Locals := l;
          Functions := functions }>
       cmd.seq
-        (cmd.call [] "ladderstep"
+        (cmd.call [] "curve_add"
                   [ expr.var X1_var; expr.var X2_var;
                   expr.var Y1_var; expr.var Y2_var;
                   expr.var Z1_var; expr.var Z2_var;
@@ -180,112 +181,36 @@ Section __.
 
   (*Why must these instances be included?*)
 
-  Instance spec_of_mul : spec_of mul.
-  Proof.
-    pose proof (binop_spec bin_mul). cbv [spec_of]. eapply X.
-  Defined.
+  Instance spec_of_mul : spec_of mul := binop_spec bin_mul.
+  Instance spec_of_add : spec_of add := binop_spec bin_add.
+  Instance spec_of_sub : spec_of sub := binop_spec bin_sub.
+  Instance spec_of_three_b : spec_of three_b_name := spec_of_from_list (feval three_b) three_b_name.
 
-  (* Instance spec_of_square : spec_of (@square field_parameters).
-  Proof.
-    pose proof (unop_spec un_square). cbv [spec_of]. eapply X.
-  Defined. *)
-
-  Instance spec_of_add : spec_of add.
-  Proof.
-    pose proof (binop_spec bin_add). cbv [spec_of]. eapply X.
-  Defined.
-
-  Instance spec_of_sub : spec_of sub.
-  Proof.
-    pose proof (binop_spec bin_sub). cbv [spec_of]. eapply X.
-  Defined.
-
-  Instance spec_of_from_list : spec_of from_list.
-  Proof.
-    pose proof (spec_of_from_list (feval three_b)). exact X.
-  Defined.
-
-  (* Instance spec_of_scmula24 : spec_of (@scmula24 prime_field_parameters).
-  Proof.
-    pose proof (unop_spec un_scmula24). cbv [spec_of]. eapply X.
-  Defined. *)
-
-  Lemma relax_bounds_FElem_R : forall R x x_ptr, Lift1Prop.impl1 ((FElem (Some tight_bounds) x_ptr x * R)%sep) ((FElem (Some loose_bounds) x_ptr x * R)%sep).
+  (* consider using seprewrite instead *)
+  Lemma relax_bounds_FElem_R : forall R x x_ptr,
+      Lift1Prop.impl1 ((FElem (Some tight_bounds) x_ptr x * R)%sep)
+        ((FElem (Some loose_bounds) x_ptr x * R)%sep).
   Proof.
     intros. cbv [Lift1Prop.impl1]. intros.
     destruct H, H, H, H0.
     eexists; eexists; split; [eapply H | ]. split; eauto. eapply relax_bounds_FElem. auto.
   Qed.
 
-  Lemma relax_bounds_binop : forall R x x_ptr y y_ptr, Lift1Prop.impl1 ((FElem (Some tight_bounds) x_ptr x * FElem (Some tight_bounds) y_ptr y * R)%sep) ((FElem (Some loose_bounds) x_ptr x * FElem (Some loose_bounds) y_ptr y * R)%sep).
-  Proof.
-    intros. cbv [Lift1Prop.impl1]. intros. eapply sep_assoc. eapply relax_bounds_FElem_R.
-    eapply sep_comm, sep_assoc. eapply relax_bounds_FElem_R. ecancel_assumption.
-  Qed.
-
   (*tactics for applying field operations*)
-
   Ltac find_in_map :=
     repeat first [ erewrite map.get_put_diff; [| intros contra; discriminate] |
       eapply map.get_put_same].
 
-  (* Local Hint Extern 8 (WeakestPrecondition.cmd _ _ _ _ _ (_ (nlet_eq _ (_ ^ 2)%F _))) =>
-    let Hsquare := (fresh "Hsquare") in pose proof compile_square as Hsquare;
-    rewrite F.pow_2_r; cbv [ Field.prime_field_parameters] in Hsquare;
-    eapply Hsquare; clear Hsquare; shelve : compiler.
-
-    Local Hint Extern 6 (WeakestPrecondition.cmd _ _ _ _ _ (_ (nlet_eq _ (a24 * _)%F _))) =>
-    let Hscmul := (fresh "Hscmul") in epose proof compile_scmula24 as Hscmul;
-    cbv [Compilation2.field_parameters Field.prime_field_parameters] in *;
-    eapply Hscmul; clear Hscmul; shelve : compiler.
-
-  Local Hint Extern 8 (WeakestPrecondition.cmd _ _ _ _ _ (_ (nlet_eq _ (_ * _)%F _))) =>
-    let Hmul := (fresh "Hmul") in pose proof compile_mul as Hmul;
-    cbv [Compilation2.field_parameters Field.prime_field_parameters] in Hmul;
-    eapply Hmul; [| | | try (eapply relax_bounds_binop; ecancel_assumption) | | |]; clear Hmul; shelve : compiler.
-
-    Local Hint Extern 8 (WeakestPrecondition.cmd _ _ _ _ _ (_ (nlet_eq _ (_ - _)%F _))) =>
-    let Hsub := (fresh "Hsub") in epose proof compile_sub as Hsub;
-    cbv [Compilation2.field_parameters Field.prime_field_parameters] in *;
-    eapply Hsub; clear Hsub; shelve : compiler.
-
-  Local Hint Extern 8 (WeakestPrecondition.cmd _ _ _ _ _ (_ (nlet_eq _ (_ + _)%F _))) =>
-    let Hadd := (fresh "Hadd") in epose proof compile_add as Hadd;
-    cbv [Compilation2.field_parameters Field.prime_field_parameters] in *;
-    eapply Hadd; clear Hadd; shelve : compiler.
-
-  Local Hint Extern 9 ((FElem (Some loose_bounds) _ _ ⋆ FElem (Some loose_bounds) _ _ ⋆ _)%sep _) =>
-    eapply relax_bounds_binop; ecancel_assumption : compiler.
-
-  Local Hint Extern 9 =>
-  simple eapply (@compile_stack _ _ _ _ _ _ _ _ _ _ _ _ _ _ _ _ _ _ _ _ _ _
-    ((@FElem width BW word mem prime_field_parameters field_representaton
-    (@None (@bounds field_parameters width BW word mem field_representaton)))));
-    [ecancel_assumption | shelve] : compiler. *)
-
-
-  Lemma FElem_bounds_None : forall x x_ptr R, Lift1Prop.impl1 (FElem (Some loose_bounds) x_ptr x * R)%sep (FElem None x_ptr x * R)%sep.
-  Proof.
-    intros. cbv [Lift1Prop.impl1]; intros m Hsep.
-    destruct Hsep as [m1 [m2 [Hsep1 [Hsep2 Hsep3]]]].
-    do 2 eexists. split; eauto. split; eauto.
-    cbv [FElem Lift1Prop.ex1] in *. sepsimpl. simpl.
-    exists x0. sepsimpl; auto.
-  Qed.
-
-  Local Hint Extern 9 ((FElem None _ _ ⋆ _ )%sep _) =>
-  eapply FElem_bounds_None; ecancel_assumption : compiler_cleanup_post.
-
-  Ltac clear_pred_seps' :=   
-  unfold pred_sep;
-  repeat change (fun x => ?h x) with h;
-  repeat match goal with
-         | [ H : _ ?m |- _ ?m] =>
-           eapply Proper_sep_impl1;
-           [ eapply P_to_bytes | clear H m; intros H m |
-            try (eapply FElem_bounds_None; ecancel_assumption);
-            try (eapply FElem_bounds_None; eapply relax_bounds_FElem_R; ecancel_assumption)]
-         end.
+  Ltac clear_pred_seps' :=
+    unfold pred_sep;
+    repeat change (fun x => ?h x) with h;
+    repeat match goal with
+      | [ H : _ ?m |- _ ?m] =>
+          eapply Proper_sep_impl1;
+          [ eapply P_to_bytes | clear H m; intros H m |
+            try (eapply drop_bounds_FElem; ecancel_assumption);
+            try (eapply drop_bounds_FElem; eapply relax_bounds_FElem_R; ecancel_assumption)]
+      end.
 
   Hint Extern 1 (pred_sep _ _ _ _ _ _) =>
          clear_pred_seps'; shelve : compiler_cleanup_post.
@@ -294,10 +219,10 @@ Section __.
          rewrite <- Hbounds_eq : compiler.
 
   Derive ladderstep_body SuchThat
-         (defn! "ladderstep" ("X1", "X2", "Y1", "Y2", "Z1", "Z2", "Xout", "Yout", "Zout")
+         (defn! "curve_add" ("X1", "X2", "Y1", "Y2", "Z1", "Z2", "Xout", "Yout", "Zout")
               { ladderstep_body },
            implements @ladderstep_gallina _ _ _ _ _ _ _ three_b
-                      using [mul; add; sub; from_list])
+                      using [mul; add; sub; three_b_name])
          As ladderstep_correct.
   Proof.
     assert (1 + 1 = 2) by lia. 
@@ -405,11 +330,13 @@ Existing Instance spec_of_ladderstep.
 Hint Extern 8 (WeakestPrecondition.cmd _ _ _ _ _ (_ (nlet_eq _ (ladderstep_gallina _ _ _ _ _ _ _) _))) =>
        simple eapply compile_ladderstep; shelve : compiler.
 
-Import Syntax.
-Local Unset Printing Coercions.
-Local Set Printing Depth 70.
+(* Import Syntax. *)
+(* Local Unset Printing Coercions. *)
+(* Local Set Printing Depth 70. *)
+
 (* Set the printing width so that arguments are printed on 1 line.
    Otherwise the build breaks.
 *)
-Local Set Printing Width 140.
-Redirect "Crypto.Bedrock.Group.ScalarMult.LadderStep.ladderstep_body" Print ladderstep_body.
+
+(* Local Set Printing Width 140. *)
+(* Redirect "Crypto.Bedrock.Group.ScalarMult.LadderStep.ladderstep_body" Print ladderstep_body. *)
