src/Bedrock/Group/CurveAdd/CurveAddAlt.v
@@ -1,8 +1,8 @@
 Require Import Rupicola.Lib.Api. Import bedrock2.WeakestPrecondition.
 Require Import Crypto.Arithmetic.PrimeFieldTheorems.
 Require Import Crypto.Bedrock.Group.CurveAdd.StoreZeroGSpec.
-Require Import Crypto.Bedrock.Specs.AbstractField.
-(* Require Import Crypto.Bedrock.Specs.PrimeField. *)
+Require Import Crypto.Bedrock.Specs.Field.
+(* Require Import Crypto.Bedrock.Specs.Field. *)
 Require Import Crypto.Bedrock.Field.Interface.CompilationAbstract.
 Require Import Crypto.Bedrock.Group.CurveAdd.CurveAdd.
 Require Import Crypto.Bedrock.Group.CurveAdd.BignumShift.
@@ -12,7 +12,101 @@ Require Import Crypto.Arithmetic.Core.
 Require Import Crypto.Arithmetic.UniformWeight.
 Local Open Scope Z_scope.
 
+(* redefining ltac *)
+(* Require Import coqutil.Macros.subst coqutil.Macros.unique bedrock2.Syntax. *)
+(* From coqutil.Tactics Require Import letexists eabstract rdelta ident_of_string. *)
+(* Require Import bedrock2.WeakestPrecondition. *)
+(* Require Import bedrock2.WeakestPreconditionProperties. *)
+(* Require Import bedrock2.Loops. *)
+(* Require Import bedrock2.Map.SeparationLogic bedrock2.Scalars. *)
+(* Import WeakestPrecondition. *)
+(* Import coqutil.Map.Interface. *)
+(* Ltac straightline_stackalloc ::= *)
+(*   match goal with Hanybytes: Memory.anybytes ?a ?n ?mStack |- _ => *)
+(*                     let m := match goal with H : map.split ?mCobined ?m mStack |- _ => m end in *)
+(*                     let mCombined := match goal with H : map.split ?mCobined ?m mStack |- _ => mCobined end in *)
+(*                     let Hsplit := match goal with H : map.split ?mCobined ?m mStack |- _ => H end in *)
+(*                     let Hm := multimatch goal with H : _ m |- _ => H end in *)
+(*                     let Hm' := fresh Hm in *)
+(*                     let Htmp := fresh in *)
+(*                     let Pm := match type of Hm with ?P m => P end in *)
+(*                     assert_fails (idtac; match goal with Halready : (Separation.sep Pm (Array.array Separation.ptsto (Interface.word.of_Z (BinNums.Zpos BinNums.xH)) a _) mCombined) |- _ => idtac end); *)
+(*                     rename Hm into Hm'; *)
+(*                     let stack := fresh "stack" in *)
+(*                     let stack_length := fresh "length_" stack in (* MUST remain in context for deallocation *) *)
+(*                     destruct (Array.anybytes_to_array_1 mStack a n Hanybytes) as (stack&Htmp&stack_length); *)
+(*                     epose proof (ex_intro _ m (ex_intro _ mStack (conj Hsplit (conj Hm' Htmp))) *)
+(*                         : Separation.sep _ (Array.array Separation.ptsto (Interface.word.of_Z (BinNums.Zpos BinNums.xH)) a _) mCombined) as Hm; *)
+(*                     clear Htmp; (* note: we could clear more here if we assumed only one separation-logic description of each memory is present *) *)
+(*                     try (let m' := fresh m in rename m into m'); rename mCombined into m; *)
+(*                     ( assert (BinInt.Z.of_nat (Datatypes.length stack) = n) *)
+(*                       by (rewrite stack_length; eauto with stack_hdb) *)
+(*                          || fail 2 "negative stackalloc of size" n ) *)
+(*   end. *)
+(* (* end redefining ltac *) *)
 
+Lemma felem_size_in_bytes_pos
+  {F : Type}
+  {width: Z}
+  {BW: Bitwidth width}
+  {word: word.word width}
+  {mem: map.map word Byte.byte}
+  {word_ok : word.ok word} {mem_ok : map.ok mem}
+  {field_parameters : FieldParameters F}
+  {field_representation : FieldRepresentation F} :
+  0 <= felem_size_in_bytes.
+Proof.
+  unfold felem_size_in_bytes.
+  pose proof bytes_per_word_range.
+  nia.
+Qed.
+
+(* Lemma FElem_equiv *)
+(*   {F : Type} *)
+(*   {width: Z} *)
+(*   {BW: Bitwidth width} *)
+(*   {word: word.word width} *)
+(*   {mem: map.map word Byte.byte} *)
+(*   {word_ok : word.ok word} {mem_ok : map.ok mem} *)
+(*   {field_parameters : FieldParameters F} *)
+(*   {field_representation : FieldRepresentation F} *)
+(*   m p x *)
+(*   : FElem (Some tight_bounds) p x m <-> (exists f, Field.FElem p f m /\ bounded_by tight_bounds f /\ feval f = x). *)
+(* Proof. *)
+(*   intros; split. *)
+(*   - intros [f]. *)
+(*     rewrite sep_emp_l in H. *)
+(*     exists f. intuition subst. *)
+(*   - intros [f]. *)
+(*     exists f. *)
+(*     rewrite sep_emp_l. *)
+(*     intuition subst. *)
+(* Qed. *)
+
+Hint Resolve felem_size_in_bytes_pos : stack_hdb.
+
+Ltac straightline_stackalloc ::=
+  match goal with Hanybytes: Memory.anybytes ?a ?n ?mStack |- _ =>
+  let m := match goal with H : map.split ?mCobined ?m mStack |- _ => m end in
+  let mCombined := match goal with H : map.split ?mCobined ?m mStack |- _ => mCobined end in
+  let Hsplit := match goal with H : map.split ?mCobined ?m mStack |- _ => H end in
+  let Hm := multimatch goal with H : _ m |- _ => H end in
+  let Hm' := fresh Hm in
+  let Htmp := fresh in
+  let Pm := match type of Hm with ?P m => P end in
+  assert_fails (idtac; match goal with Halready : (Separation.sep Pm (Array.array Separation.ptsto (Interface.word.of_Z (BinNums.Zpos BinNums.xH)) a _) mCombined) |- _ => idtac end);
+  rename Hm into Hm';
+  let stack := fresh "stack" in
+  let stack_length := fresh "length_" stack in (* MUST remain in context for deallocation *)
+  destruct (Array.anybytes_to_array_1 mStack a n Hanybytes) as (stack&Htmp&stack_length);
+  epose proof (ex_intro _ m (ex_intro _ mStack (conj Hsplit (conj Hm' Htmp)))
+  : Separation.sep _ (Array.array Separation.ptsto (Interface.word.of_Z (BinNums.Zpos BinNums.xH)) a _) mCombined) as Hm;
+  clear Htmp; (* note: we could clear more here if we assumed only one separation-logic description of each memory is present *)
+  try (let m' := fresh m in rename m into m'); rename mCombined into m;
+  assert (BinInt.Z.of_nat (Datatypes.length stack) = n)
+  by (rewrite stack_length, Z2Nat.id; eauto with stack_hdb
+  || fail 2 "negative stackalloc of size" n )
+  end.
 
 Section __.
   Context {width: Z} {BW: Bitwidth width} {word: word.word width} {mem: map.map word Byte.byte}.
@@ -23,30 +117,32 @@ Section __.
   Context {locals_ok : map.ok locals}.
   Context {env_ok : map.ok env}.
   Context {ext_spec_ok : Semantics.ext_spec.ok ext_spec}.
-  Context {field_parameters : AbstractField.FieldParameters}
-          {field_parameters_ok : AbstractField.FieldParameters_ok}.
+  Context {F : Type} {field_parameters : Field.FieldParameters F}
+          {field_parameters_ok : Field.FieldParameters_ok F}.
+  Context {field_names : FieldNames F}.
   
-  Context {field_representation : FieldRepresentation}
-          {field_representation_ok : FieldRepresentation_ok}
+  Context {field_representation : FieldRepresentation F}
+          {field_representation_ok : FieldRepresentation_ok F}
           {curve_add_alt : string}.
 
   Hint Resolve relax_bounds : compiler.
-  Instance my_field_representation : FieldRepresentation.
-  Proof.
-      exact field_representation.
-  Defined.
+  (* Instance my_field_representation : FieldRepresentation F. *)
+  (* Proof. *)
+  (*     exact field_representation. *)
+  (* Defined. *)
 
   Context (three_b : felem).
 
-  Instance spec_of_felem_copy : spec_of "felem_copy".
-  Proof.
-     pose proof spec_of_felem_copy. eapply X.
-   Defined.
 
-   Instance spec_of_curve_add : spec_of "curve_add".
-   Proof.
-      pose proof spec_of_ladderstep. specialize (X three_b). exact X.
-   Defined.
+  Instance spec_of_felem_copy : spec_of "felem_copy" := spec_of_felem_copy.
+  (* Proof. *)
+  (*    pose proof spec_of_felem_copy. eapply X. *)
+  (*  Defined. *)
+
+   Instance spec_of_curve_add : spec_of "curve_add" := spec_of_ladderstep three_b.
+   (* Proof. *)
+   (*    pose proof spec_of_ladderstep. specialize (X three_b). exact X. *)
+   (* Defined. *)
 
   Instance spec_of_curve_add_alt : spec_of curve_add_alt :=
   fnspec! curve_add_alt
@@ -65,18 +161,25 @@ Section __.
        * FElem (Some tight_bounds) pYout Youtold
        * FElem (Some tight_bounds) pZout Zoutold * Rout)%sep mem;
     ensures tr' mem' :=
+      tr = tr' /\
          exists Xout Yout Zout (* output values *)
                 : F ,
-                (@ladderstep_gallina _ _ _ _ _ _ three_b X1 X2 Y1 Y2 Z1 Z2
+                (@ladderstep_gallina _ _ _ _ _ _ _ three_b X1 X2 Y1 Y2 Z1 Z2
          = \<Xout, Yout, Zout\>)
         /\
+          (* (FElem (Some tight_bounds) pX1 X1 *)
+          (*       * FElem (Some tight_bounds) pX2 X2 *)
+          (*       * FElem (Some tight_bounds) pY1 Y1 *)
+          (*       * FElem (Some tight_bounds) pY2 Y2 *)
+          (*       * FElem (Some tight_bounds) pZ1 Z1 *)
+          (*       * FElem (Some tight_bounds) pZ2 Z2 *)
         (* (FElem (Some tight_bounds) pX1 X1
               * FElem (Some tight_bounds) pY1 Y1
               * FElem (Some tight_bounds) pZ1 Z1 * R1)%sep mem' /\
            (FElem (Some tight_bounds) pX2 X2
               * FElem (Some tight_bounds) pY2 Y2
               * FElem (Some tight_bounds) pZ2 Z2 * R2)%sep mem' /\ *)
-           (FElem (Some tight_bounds) pXout Xout
+              (FElem (Some tight_bounds) pXout Xout
               * FElem (Some tight_bounds) pYout Yout
               * FElem (Some tight_bounds) pZout Zout * Rout)%sep mem'}.
 
@@ -85,40 +188,83 @@ Section __.
    Import Syntax BinInt String List.ListNotations.
    Local Open Scope string_scope. Local Open Scope Z_scope. Local Open Scope list_scope.
 
+
    Definition curve_add_alt_func : bedrock2.Syntax.func :=
-   ("curve_add_alt", (["px1"; "px2"; "py1"; "py2"; "pz1"; "pz2"; "outx"; "outy"; "outz"], []:list String.string, bedrock_func_body:(
-      stackalloc 48 as px1a;
-      stackalloc 48 as py1a;
-      stackalloc 48 as pz1a;
-      stackalloc 48 as px2a;
-      stackalloc 48 as py2a;
-      stackalloc 48 as pz2a;
-      coq:(cmd.call [] ("felem_copy") [expr.var ("px1a"); expr.var ("px1")]);
-      coq:(cmd.call [] ("felem_copy") [expr.var ("px2a"); expr.var ("px2")]);
-      coq:(cmd.call [] ("felem_copy") [expr.var ("py1a"); expr.var ("py1")]);
-      coq:(cmd.call [] ("felem_copy") [expr.var ("py2a"); expr.var ("py2")]);
-      coq:(cmd.call [] ("felem_copy") [expr.var ("pz1a"); expr.var ("pz1")]);
-      coq:(cmd.call [] ("felem_copy") [expr.var ("pz2a"); expr.var ("pz2")]);
-      coq:(cmd.call [] ("curve_add") [expr.var ("px1"); expr.var ("px2"); expr.var ("py1"); expr.var ("py2"); expr.var ("pz1"); expr.var ("pz2"); expr.var ("outx"); expr.var ("outy"); expr.var ("outz")])
+   (curve_add_alt, (["px1"; "px2"; "py1"; "py2"; "pz1"; "pz2"; "outx"; "outy"; "outz"], []:list String.string, bedrock_func_body:(
+      stackalloc felem_size_in_bytes as px1a;
+      stackalloc felem_size_in_bytes as py1a;
+      stackalloc felem_size_in_bytes as pz1a;
+      stackalloc felem_size_in_bytes as px2a;
+      stackalloc felem_size_in_bytes as py2a;
+      stackalloc felem_size_in_bytes as pz2a;
+      coq:(cmd.call [] (felem_copy) [expr.var ("px1a"); expr.var ("px1")]);
+      coq:(cmd.call [] (felem_copy) [expr.var ("px2a"); expr.var ("px2")]);
+      coq:(cmd.call [] (felem_copy) [expr.var ("py1a"); expr.var ("py1")]);
+      coq:(cmd.call [] (felem_copy) [expr.var ("py2a"); expr.var ("py2")]);
+      coq:(cmd.call [] (felem_copy) [expr.var ("pz1a"); expr.var ("pz1")]);
+      coq:(cmd.call [] (felem_copy) [expr.var ("pz2a"); expr.var ("pz2")]);
+      coq:(cmd.call [] ("curve_add") [expr.var ("px1a"); expr.var ("px2a"); expr.var ("py1a"); expr.var ("py2a"); expr.var ("pz1a"); expr.var ("pz2a"); expr.var ("outx"); expr.var ("outy"); expr.var ("outz")])
    ))).
 
-    From bedrock2 Require Import ToCString Bytedump.
-    Definition c_mod := (c_module (curve_add_alt_func :: nil)).
-    Eval native_compute in c_mod.
+    (* From bedrock2 Require Import ToCString Bytedump. *)
+    (* Definition c_mod := (c_module (curve_add_alt_func :: nil)). *)
+    (* Eval native_compute in c_mod. *)
 
-    Print c_mod.
+   Opaque felem_size_in_bytes.
+    (* Print c_mod. *)
 
-   Ltac solve_locals7 l5 l4 l3 l2 l1 l0 l :=
-      subst l5 l4 l3 l2 l1 l0 l; repeat (erewrite map.get_put_diff; [| intros contra; discriminate]); eapply map.get_put_same.
+   Ltac collect H1 H2 H3 := let Hnew := (fresh "Hnew") in
+                            eassert (Hnew : id (fun m => (_ m) /\ (_ m) /\ (_ m)) _) by (cbv [id]; repeat split; [eapply H1| eapply H2|eapply H3]); clear H1 H2 H3.
 
-   Ltac solve_locals6 l4 l3 l2 l1 l0 l :=
-      subst l4 l3 l2 l1 l0 l; repeat (erewrite map.get_put_diff; [| intros contra; discriminate]); eapply map.get_put_same.
+   Ltac update_mem :=
+     match goal with
+     | Hsplit : map.split ?comb ?mem ?stack |- _ =>
+         match goal with
+           Hold_mem : ?p mem,
+             Hstack : Memory.anybytes ?a felem_size_in_bytes stack
+           |- _ =>
+             let x := fresh "x" in
+             let Hmem := fresh "Hmem" in
+             eapply FElem_from_bytes in Hstack as [x Hstack]
+             ; eassert (Hnew_mem : (p ⋆ FElem None a x) comb) by (eexists; eauto)
+             ; clear dependent mem
+             ; clear dependent stack
+             ; rename Hnew_mem into Hmem
+         end
+     end.
 
+  Ltac straightline' :=
+    match goal with
+    | _ => update_mem
+    | _ => straightline
+    | l := _ : map.rep |- _ => subst l
+    | l := _ : list word.rep |- _ => subst l
+    | |- Some _ = Some _ => try reflexivity
+    | |- exists _, _ => eexists
+    | |- _ /\ _ => split
+    | |- felem_size_in_bytes mod _ = 0 => eapply felem_size_in_bytes_mod
+    | |- map.get _ _ = _ => repeat (erewrite map.get_put_diff; [| intros contra; discriminate]); eapply map.get_put_same
+    end.
+
+  Ltac sep_and_fwd :=
+    cbn [id] in *;
+    match goal with
+    | H : context[fun m => _] |- _ =>
+        let Hnew1 := fresh "Hmem" in
+        let Hnew2 := fresh "Hmem" in
+        eassert (Hnew1 : ((fun m => _) ⋆ _) _) by ecancel_assumption;
+        eapply sep_and_l_fwd in Hnew1 as [Hnew1 Hnew2];
+        clear H
+    end.
+
+  Instance spec_of_F_felem_copy : spec_of felem_copy := spec_of_felem_copy.
 
    Lemma curve_add_alt_ok : program_logic_goal_for_function! curve_add_alt_func.
    Proof.
       enter curve_add_alt_func.
-      repeat straightline.
+
+      repeat straightline'.
+      (* cbv [curve_add_alt]. *)
 
       remember ((FElem (Some tight_bounds) pX1 X1 ⋆ FElem (Some tight_bounds) pY1 Y1
       ⋆ FElem (Some tight_bounds) pZ1 Z1 ⋆ R1))%sep as P1.
@@ -130,165 +276,245 @@ Section __.
       ⋆ FElem (Some tight_bounds) pYout Youtold
       ⋆ FElem (Some tight_bounds) pZout Zoutold ⋆ Rout))%sep as P3.
 
-      assert ( (fun m => (P1 m /\ P2 m /\ P3 m)) mem0) by auto.
-      clear H8 H7 H6.
+      (* assert (id ((fun m => (P1 m /\ P2 m /\ P3 m)) mem0)) by (simpl; auto). *)
+      (* clear H8 H7 H6. *)
+
+      (* rewrite String.eqb_refl. *)
+      (* clear H0 H1 H2 H3 H4. *)
+      (* do 3 straightline'. *)
+      collect H6 H7 H8.
+      (* rename H0 into Hmem. *)
+      (* clear H6 H7 H8. *)
+      repeat straightline'.
 
       simpl.
-      assert (curve_add_alt =? curve_add_alt = true)%string.
-      {
-         eapply String.eqb_eq. auto.
-      }
-      rewrite H6.
-      eexists; split; [cbv [map.of_list_zip]; simpl; eauto| ].
+      rewrite String.eqb_refl.
+      repeat straightline'.
 
-      remember  (fun m : mem => P1 m /\ P2 m /\ P3 m) as eyy.
+      (* eassert (Htemp : forall m, array ptsto (word.of_Z 1) a stack17 m <-> exists f, Field.FElem a f m). *)
+      (* intros. split. *)
+      (* { admit. } *)
+      (*   (* intros. eapply array_1_to_anybytes in H65. *) *)
+      (*   (* pose proof alloc_to_FElem a m. *) *)
+
+      (*   (* exists (Util.encode_bytes stack17). *) *)
+      (*   (* split. *) *)
+      (*   (* eapply alloc_to_FElem. rewrite <- H54. assumption. } *) *)
+      (* { intros. pose proof anybytes_to_array_1 m a felem_size_in_bytes. *)
+      (*   destruct H65 as [f]. *)
+      (*   eapply FElem_to_anybytes in H65. *)
+      (*   apply H66 in H65 as []. *)
+      (* } *)
+      (* try destruct Htemp. try rewrite H65 in *. *)
+
+      (* try eassert (Htemp : exists f, array ptsto (word.of_Z 1) a0 stack18 = Field.FElem a f) by admit. *)
+      (* try destruct Htemp. try rewrite H66 in *. *)
+
+      (* try eassert (Htemp : exists f, array ptsto (word.of_Z 1) a1 stack19 = Field.FElem a f) by admit. *)
+      (* try destruct Htemp. try rewrite H67 in *. *)
+
+      (* try eassert (Htemp : exists f, array ptsto (word.of_Z 1) a2 stack20 = Field.FElem a f) by admit. *)
+      (* try destruct Htemp. try rewrite H68 in *. *)
+
+      (* try eassert (Htemp : exists f, array ptsto (word.of_Z 1) a3 stack21 = Field.FElem a f) by admit. *)
+      (* try destruct Htemp. try rewrite H69 in *. *)
+
+      (* try eassert (Htemp : exists f, array ptsto (word.of_Z 1) a4 stack22 = Field.FElem a f) by admit. *)
+      (* try destruct Htemp. try rewrite H70 in *. *)
+      (* assert (Hequiv : forall p x, exists f, FElem (Some tight_bounds) p x = emp (bounded_by tight_bounds f /\ feval f = x) ⋆ (Field.FElem p f)). *)
+      (* intros. *)
+      (* destruct (FElem (Some tight_bounds) p x). *)
+      (* pose proof FElem_equiv mem0 pX1 X1. *)
+      (* rewrite H65 in H10. *)
+
+      (* rewrite (FElem_equiv) in H10. *)
+      (* eassert (Htemp : forall m, FElem (Some tight_bounds) pX1 X1 m <-> (exists f, Field.FElem pX1 f m /\ bounded_by tight_bounds f /\ feval f = X1)). *)
+      (* intros; split. *)
+      (* { intros. destruct H65 as [f]. *)
+      (*   rewrite sep_emp_l in H65. *)
+      (*   unfold maybe_bounded in H65. *)
+      (*   exists f. intuition subst. } *)
+      (* { intros [f]. *)
+      (*   exists f. *)
+      (*   rewrite sep_emp_l. *)
+      (* intuition subst. } *)
+
+      (* eauto. *)
+      (*   eauto. *)
+      (*   sep eauto. assumption. } *)
+      (* try destruct Htemp, H71, H72. try rewrite H71 in *. *)
+
+      (* try eassert (Htemp : exists f, FElem (Some tight_bounds) pX2 X2 = Field.FElem pX2 f /\ bounded_by tight_bounds f /\ feval f = X2) by admit. *)
+      (* try destruct Htemp, H73, H74. try rewrite H73 in *. *)
+
+      (* try eassert (Htemp : exists f, FElem (Some tight_bounds) pY1 Y1 = Field.FElem pY1 f /\ bounded_by tight_bounds f /\ feval f = Y1) by admit. *)
+      (* try destruct Htemp, H75, H76. try rewrite H75 in *. *)
+
+      (* try eassert (Htemp : exists f, FElem (Some tight_bounds) pY2 Y2 = Field.FElem pY2 f /\ bounded_by tight_bounds f /\ feval f = Y2) by admit. *)
+      (* try destruct Htemp, H77, H78. try rewrite H77 in *. *)
+
+      (* try eassert (Htemp : exists f, FElem (Some tight_bounds) pZ1 Z1 = Field.FElem pZ1 f /\ bounded_by tight_bounds f /\ feval f = Z1) by admit. *)
+      (* try destruct Htemp, H79, H80. try rewrite H79 in *. *)
+
+      straightline_call.
+      {
+        (* simpl in Hmem. *)
+        split.
+        (* NB: In goal 2, doing sep_and_fwd first does not preserve all memory for after the call (it uses the wrong ambient memory for FElem None a out) *)
+        2: ecancel_assumption.
+        do 2 sep_and_fwd.
+        subst P1 P2 P3.
+        ecancel_assumption.
+      }
+      clear dependent mCombined0.
+
+      repeat straightline'.
+
+      straightline_call.
+      {
+        repeat split.
+        2: ecancel_assumption.
+        repeat sep_and_fwd.
+        subst P1 P2 P3.
+        ecancel_assumption.
+      }
+      clear dependent a6.
+
+      repeat straightline'.
+
+      straightline_call.
+      {
+        repeat split.
+        2: ecancel_assumption.
+        repeat sep_and_fwd.
+        subst P1 P2 P3.
+        ecancel_assumption.
+      }
+      clear dependent a8.
+
+      repeat straightline'.
+
+      straightline_call.
+      {
+        repeat split.
+        2: ecancel_assumption.
+        repeat sep_and_fwd.
+        subst P1 P2 P3.
+        ecancel_assumption.
+      }
+      clear dependent a6.
+
+      repeat straightline'.
+
+      straightline_call.
+      {
+        repeat split.
+        2: ecancel_assumption.
+        repeat sep_and_fwd.
+        subst P1 P2 P3.
+        ecancel_assumption.
+      }
+      clear dependent a8.
+
+      repeat straightline'.
+
+      straightline_call.
+      {
+        repeat split.
+        2: ecancel_assumption.
+        repeat sep_and_fwd.
+        subst P1 P2 P3.
+        ecancel_assumption.
+      }
+      clear dependent a6.
+
+      repeat straightline'.
+
+      straightline_call.
+      {
+        repeat split.
+        (* 2: ecancel_assumption. *)
+        repeat sep_and_fwd.
+        subst P3.
+        ecancel_assumption.
+      }
+      clear dependent a8.
 
       repeat straightline.
-
+      eexists.
       split.
-      {
-         admit.
+      straightline'.
+      straightline'.
+      straightline'.
+      reflexivity.
+
+      eassert (h1 : (FElem _ a4 _ ⋆ _) a6) by ecancel_assumption.
+
+      destruct h1 as [mq [mr [h1 [h2 h3]]]].
+
+      eexists. eexists. split.
+      1: {
+        eapply FElem_from_bytes. eexists. eapply drop_bounds_FElem. eauto.
       }
+      split; [eapply map.split_comm; eauto| ].
 
-      repeat straightline.
+      eassert (h4 : (FElem _ a3 _ ⋆ _) mr) by ecancel_assumption.
 
-      split.
-      {
-         admit.
-      }
+    destruct h4 as [mq' [mr' [h4 [h5 h6]]]].
 
-      repeat straightline.
-      split.
-      {
-         admit.
-      }
+    eexists. eexists. split.
+    1: {
+      eapply FElem_from_bytes. eexists. eapply drop_bounds_FElem. eauto.
+    }
+    split; [eapply map.split_comm; eauto| ].
 
-      repeat straightline. split.
-      {
-         admit.
-      }
+    eassert (h7 : (FElem _ a2 _ ⋆ _) mr') by ecancel_assumption.
 
-      repeat straightline.
+    destruct h7 as [mq'' [mr'' [h7 [h8 h9]]]].
+    eexists. eexists. split.
+    1: {
+      eapply FElem_from_bytes. eexists. eapply drop_bounds_FElem. eauto.
+    }
+    split; [eapply map.split_comm; eauto| ].
 
-      split.
-      {
-         admit.
-      }
+    eassert (h10 : (FElem _ a1 _ ⋆ _) mr'') by ecancel_assumption.
 
-      repeat straightline. split.
-      {
-         admit.
-      }
+    destruct h10 as [mq''' [mr''' [h10 [h11 h12]]]].
+    eexists. eexists. split.
+    1: {
+      eapply FElem_from_bytes. eexists. eapply drop_bounds_FElem. eauto.
+    }
+    split; [eapply map.split_comm; eauto| ].
 
-      
-      repeat straightline.
+    eassert (h13 : (FElem _ a0 _ ⋆ _) mr''') by ecancel_assumption.
 
-      eexists. split.
-      {
-         repeat straightline. eexists. split; [solve_locals6 l4 l3 l2 l1 l0 l| ].
-         repeat straightline. eexists. split; [solve_locals6 l4 l3 l2 l1 l0 l| ].
-         repeat straightline.
-      }
+    destruct h13 as [mq'''' [mr'''' [h13 [h14 h15]]]].
+    eexists. eexists. split.
+    1: {
+      eapply FElem_from_bytes. eexists. eapply drop_bounds_FElem. eauto.
+    }
+    split; [eapply map.split_comm; eauto| ].
 
-      repeat straightline. clear H30 H26 H22 H18 H14.
-      subst eyy P1 P2 P3.
-      repeat straightline.
+    eassert (h16 : (FElem _ a _ ⋆ _) mr'''') by ecancel_assumption.
 
-      eassert (Htemp : exists f, array ptsto (word.of_Z 1) a stack17 = AbstractField.FElem a f) by admit.
-      destruct Htemp. rewrite H65 in *.
+    destruct h16 as [mq''''' [mr''''' [h16 [h17 h18]]]].
+    eexists. eexists. split.
+    1: {
+      eapply FElem_from_bytes. eexists. eapply drop_bounds_FElem. eauto.
+    }
+    split; [eapply map.split_comm; eauto| ].
 
-      eassert (Htemp : exists f, array ptsto (word.of_Z 1) a0 stack18 = AbstractField.FElem a f) by admit.
-      destruct Htemp. rewrite H66 in *.
+    split; auto.
 
-      eassert (Htemp : exists f, array ptsto (word.of_Z 1) a1 stack19 = AbstractField.FElem a f) by admit.
-      destruct Htemp. rewrite H67 in *.
+    split; auto.
 
-      eassert (Htemp : exists f, array ptsto (word.of_Z 1) a2 stack20 = AbstractField.FElem a f) by admit.
-      destruct Htemp. rewrite H68 in *.
+    do 3 eexists.
+    split.
+    eassumption.
 
-      eassert (Htemp : exists f, array ptsto (word.of_Z 1) a3 stack21 = AbstractField.FElem a f) by admit.
-      destruct Htemp. rewrite H69 in *.
+    ecancel_assumption.
 
-      eassert (Htemp : exists f, array ptsto (word.of_Z 1) a4 stack22 = AbstractField.FElem a f) by admit.
-      destruct Htemp. rewrite H70 in *.
-
-      eassert (Htemp : exists f, FElem (Some tight_bounds) pX1 X1 = AbstractField.FElem pX1 f /\ bounded_by tight_bounds f /\ feval f = X1) by admit.
-      destruct Htemp, H71, H72. rewrite H71 in *.
-
-      eassert (Htemp : exists f, FElem (Some tight_bounds) pX2 X2 = AbstractField.FElem pX2 f /\ bounded_by tight_bounds f /\ feval f = X2) by admit.
-      destruct Htemp, H73, H74. rewrite H73 in *.
-
-      eassert (Htemp : exists f, FElem (Some tight_bounds) pY1 Y1 = AbstractField.FElem pY1 f /\ bounded_by tight_bounds f /\ feval f = Y1) by admit.
-      destruct Htemp, H75, H76. rewrite H75 in *.
-
-      eassert (Htemp : exists f, FElem (Some tight_bounds) pY2 Y2 = AbstractField.FElem pY2 f /\ bounded_by tight_bounds f /\ feval f = Y2) by admit.
-      destruct Htemp, H77, H78. rewrite H77 in *.
-
-      eassert (Htemp : exists f, FElem (Some tight_bounds) pZ1 Z1 = AbstractField.FElem pZ1 f /\ bounded_by tight_bounds f /\ feval f = Z1) by admit.
-      destruct Htemp, H79, H80. rewrite H79 in *.
-
-
-
-
-
-
-      eapply Proper_call.
-      2: {
-         pose proof H. cbv [spec_of_felem_copy AbstractField.spec_of_felem_copy] in H82.
-         assert (felem_copy = "felem_copy") by admit.
-         rewrite H83 in H82.
-         eapply H82. split; cbv [my_field_representation].
-         1: {
-            cbv [my_field_representation] in *.
-             ecancel_assumption.
-         }
-         cbv [my_field_representation] in *. ecancel_assumption.
-      }
-
-       clear H63 H61 H59 H57  H55 H51  H49 H47 H45 H43 H39 H37 H35 H33 H30.
-
-      cbv [pointwise_relation Basics.impl]. intros.
-      destruct H30.
-
-      eexists. split.
-      {
-         subst 
-      }
-
-             eassert ((AbstractField.FElem pX1 x5 * AbstractField.FElem a x0 * _)%sep mem0).
-             {
-                cbv [my_field_representation] in *.
-                ecancel_assumption.
-             }
-             eapply H85.
-             
-             ecancel_assumption.
-             Set Printing All.
-
-             cbv [my_field_representation] in *.
-             ecancel_assumption.
-            rewrite H68.
-
-
-            Set Printing All.
-            Lemma forall p x
-
-         }
-         1: ecancel_assumption.
-         pose proof H9.
-         
-         ecancel_assumption.
-         ecancel_assumption.
-      }
-
-      repeat straightline.
-
-
-
-      repeat straightline.
-      split; [admit| ].
-      compile_step.
-
+   Qed.
 
 
 
