src/Bedrock/Group/CurveAdd/Test.v
@@ -1,142 +1,84 @@
 Require Import Crypto.Bedrock.Field.Synthesis.Examples.bls12_prime.
-Require Import Crypto.Bedrock.Field.Synthesis.Examples.bls12_from_list_F.
-Require Import Crypto.Bedrock.Group.CurveAdd.StorePointAtInfinity.
-Require Import Crypto.Bedrock.Field.Synthesis.Examples.BLS12_G1.
-Require Import Crypto.Bedrock.Field.Synthesis.Examples.BLS12_G1_alt.
+Require Import Crypto.Bedrock.Group.CurveAdd.StoreZero.
 Require Import Crypto.Bedrock.Group.CurveAdd.BignumShift.
 Require Import Crypto.Bedrock.Group.CurveAdd.CondMoveGroup.
+Require Import Crypto.Bedrock.Group.CurveAdd.CurveAdd.
 Require Import Crypto.Bedrock.Group.CurveAdd.CurveAddAlt.
 (* why is this called p224? *)
-Require Import Crypto.Bedrock.Field.Synthesis.Examples.felem_copy_p224.
+Require Import Crypto.Bedrock.Field.Synthesis.Examples.bls12_felem_copy.
+(* this should be named "something three_b" *)
+Require Import Crypto.Bedrock.Field.Synthesis.Examples.bls12_from_list_F.
 Require Import Crypto.Bedrock.Group.CurveAdd.LoopBody.
 Require Import Crypto.Bedrock.Group.CurveAdd.ScalarMult.
 
-     (* Require Import bedrock2.Syntax. *)
-     (* Require Import compiler.MMIO. *)
+Require Import compiler.Pipeline.
+From bedrock2 Require Import ToCString Bytedump.
 
-     Require Import compiler.Pipeline.
-     From bedrock2 Require Import ToCString Bytedump.
+Require Import bedrock2.Syntax.
+Require Import compiler.MMIO.
 
-     Require Import bedrock2.Syntax.
-     Require Import compiler.MMIO.
-     Definition funcs : list func :=
-       [ bls12_select_znz].
-
-     Compute compile (compile_ext_call (funname_env:=SortedListString.map)) (map.of_list funcs).
 Import Syntax BinInt String List.ListNotations.
 Local Open Scope string_scope. Local Open Scope Z_scope. Local Open Scope list_scope.
 Local Open Scope sep_scope.
 
+From bedrock2 Require Import ToCString Bytedump.
 
 Existing Instance bls12_field_names.
+Existing Instance bls12_prime_parameters.
+Existing Instance bls12_field_parameters.
+Existing Instance bls12_field_representation.
 
-From bedrock2 Require Import ToCString Bytedump.
-Definition c_mod := (c_module (store_zero_func:: nil)).
-(* Definition mul_fun := Eval vm_compute in (bls12_mul). *)
-(* Definition mul_fun := Eval vm_compute in (bls12_mul). *)
-Eval compute in bls12_select_znz.
-(* Eval compute in cmov_func (group_cmov:="group_cmov"). *)
+(* for debugging *)
+Definition bls12_add_mod := (c_module (bls12_add :: nil)).
+Eval compute in bls12_add_mod.
+Definition bls12_mul_mod := (c_module (bls12_mul :: nil)).
+(* slow *)
+(* Eval compute in bls12_mul_mod. *)
+Definition bls12_zero_mod := (c_module (bls12_zero :: nil)).
+Eval compute in bls12_zero_mod.
+Definition bls12_one_mod := (c_module (bls12_one :: nil)).
+Eval compute in bls12_one_mod.
+Definition bls12_select_znz_mod := (c_module (bls12_select_znz :: nil)).
+Eval compute in bls12_select_znz_mod.
+Definition felem_copy_mod := (c_module (felem_copy_func :: nil)).
+Eval compute in felem_copy_mod.
+Definition store_zero_mod := (c_module (store_zero_func :: nil)).
+Eval compute in store_zero_mod.
+Definition shift_scalar_mod := (c_module (shift_scalar (width:=64) :: nil)).
+Eval compute in shift_scalar_mod.
+
+(* the names instantiated here should be collected in a GroupNames typeclass *)
+(* also, they should parametrized in all implementations
+   e.g. "group_cmov" is hardcoded in loop_body *)
+Definition three_b_func_mod := (c_module (bls12_three_b :: nil)).
+Eval compute in three_b_func_mod.
+Definition cmov_alt_func_mod := (c_module (cmov_alt_func (group_cmov_alt:="group_cmov_alt") :: nil)).
+Eval compute in cmov_alt_func_mod.
+Definition curve_add_mod := (c_module (ladderstep_body "bls12_three_b" :: nil)).
+Eval compute in curve_add_mod.
+Definition curve_add_alt_mod := (c_module (curve_add_alt_func (curve_add_alt:="curve_add_alt") :: nil)).
+Eval compute in curve_add_alt_mod.
+Definition loop_body_func_mod := (c_module (loop_body_func "curve_add_alt" :: nil)).
+Eval compute in loop_body_func_mod.
+Definition scalar_mult_func_mod := (c_module (scalar_mult_func (scalar_words:=4) :: nil)).
+Eval compute in scalar_mult_func_mod.
 
 Definition c_test :=
   Eval vm_compute in
     c_module (bls12_add
                 :: bls12_sub
                 :: bls12_mul
-                :: bls12_from_list
-                :: bls12_G1_add
-                :: felem_copy_func
-                :: G1_add_alt
                 :: bls12_zero
                 :: bls12_one
-                :: store_zero_func
-                :: shift_scalar
                 :: bls12_select_znz
-                :: cmov_func (group_cmov:="group_cmov") (* set the name somewhere consistent *)
-                :: (loop_body_func "G1_add_alt")
-                :: scalar_mult_func
+                :: felem_copy_func
+                :: store_zero_func
+                :: shift_scalar (width:=64)
+                :: bls12_three_b
+                :: cmov_alt_func (group_cmov_alt:="group_cmov_alt") (* set the name somewhere consistent *)
+                :: ladderstep_body "bls12_three_b"
+                :: curve_add_alt_func (curve_add_alt:="curve_add_alt")
+                :: (loop_body_func "curve_add_alt")
+                :: scalar_mult_func (scalar_words:=4)
                 :: nil).
 Redirect "c_test" Eval cbv in c_test.
-
-(* Local Open Scope bytedump_scope. *)
-(* Import Syntax BinInt String List.ListNotations. *)
-(* Local Open Scope string_scope. *)
-(* Local Open Scope Z_scope. *)
-(* Local Open Scope list_scope. *)
-Require Import Crypto.Bedrock.Field.Synthesis.Examples.bls12_prime.
-Require Import Crypto.Bedrock.Field.Synthesis.Examples.BLS12_G1.
-(* Require Import Crypto.Bedrock.Field.Synthesis.Examples.bls12_from_list_F. *)
-Require Import Crypto.Bedrock.Group.CurveAdd.StorePointAtInfinity.
-
-Section test.
-
-  (* Existing Instance bls12_field_names. *)
-  (* Existing Instance bls12_field_parameters. *)
-  (* Existing Instance bls12_field_representation. *)
-
-  (* Definition three_b := 0. *)
-  (*   Definition uw := (uweight 64). *)
-  (*   Definition n := felem_size_in_words. *)
-  (*   Definition three_b_list := Partition.partition uw n three_b. *)
-  (*   Definition word := BasicC64Semantics.word. *)
-  (*   Definition three_b_mont := Eval vm_compute in (@WordByWordMontgomery.to_montgomerymod 64 n m (@m' bls12_prime.field_parameters 64) three_b_list). *)
-  (*   Definition three_b_words := List.map (@word.of_Z 64 word) three_b_mont. *)
-
-  (*     Instance spec_of_store_zero : spec_of "store_zero_G" := *)
-  (*     fnspec! "store_zero_G" *)
-  (*           (pX pY pZ: word) *)
-  (*           / (X Y Z : F) R, *)
-  (*     { requires tr mem := *)
-  (*           (FElem (Some tight_bounds) pX X *)
-  (*           * FElem (Some tight_bounds) pY Y *)
-  (*           * FElem (Some tight_bounds) pZ Z * R)%sep mem; *)
-  (*           ensures tr' mem' := *)
-  (*                 (FElem (Some tight_bounds) pX Fzero *)
-  (*           * FElem (Some tight_bounds) pY Fone *)
-  (*           * FElem (Some tight_bounds) pZ Fzero * R)%sep mem'}. *)
-
-          (* Definition from_list_func : Syntax.func := ("store_zero_F", (["out"], (nil : list string), bedrock_func_body:(
-                coq:(cmd.store access_size.word (expr.var "out") (expr.literal (nth 0 three_b_mont 0)));
-                coq:(cmd.store access_size.word (expr.op bopname.add (expr.var "out") (expr.literal (8))) (nth 1 three_b_mont 0));
-                coq:(cmd.store access_size.word (expr.op bopname.add (expr.var "out") (expr.literal (16))) (nth 2 three_b_mont 0));
-                coq:(cmd.store access_size.word (expr.op bopname.add (expr.var "out") (expr.literal (24))) (nth 3 three_b_mont 0));
-                coq:(cmd.store access_size.word (expr.op bopname.add (expr.var "out") (expr.literal (32))) (nth 4 three_b_mont 0));
-                coq:(cmd.store access_size.word (expr.op bopname.add (expr.var "out") (expr.literal (40))) (nth 5 three_b_mont 0))
-              ))).
-
-        Definition store_zero_func : bedrock2.Syntax.func :=
-        ("store_zero", (["outx"; "outy"; "outz"], []:list String.string, bedrock_func_body:(
-                coq:(cmd.call [] "store_zero_F" [expr.var ("outx")]);
-                coq:(cmd.call [] "store_one_F" [expr.var ("outy")]);
-                coq:(cmd.call [] "store_zero_F" [expr.var ("outz")])
-        ))).
-
-        From bedrock2 Require Import ToCString Bytedump.
-        Definition c_mod := (c_module (store_zero_func:: nil)).
-
-        Eval native_compute in c_mod. *)
-
-
-Import Syntax BinInt String List.ListNotations.
-Local Open Scope string_scope. Local Open Scope Z_scope. Local Open Scope list_scope.
-
-From bedrock2 Require Import ToCString Bytedump.
-Definition c_mod := (c_module (bls12_G1_add :: nil)).
-Eval native_compute in c_mod.
-
-    Existing Instances Defaults64.default_parameters Defaults64.default_parameters_ok.
-
-    (* Local Notation F := (F M_pos). *)
-
-    Check CurveAdd.ladderstep_body.
-
-    Existing Instance bls12_prime_parameters.
-    Existing Instance bls12_field_names.
-    Existing Instance bls12_field_parameters.
-    Existing Instance WordByWordMontgomery.field_representation.
-Import Syntax BinInt String List.ListNotations.
-Local Open Scope string_scope. Local Open Scope Z_scope. Local Open Scope list_scope.
-
-From bedrock2 Require Import ToCString Bytedump.
-Definition c_mod := (c_module (bls12_G1_add :: nil)).
-
-Eval native_compute in c_mod.
